Weidenbach_Book/IsaSAT/IsaSAT_Setup1_LLVM.thy
@@ -1,5 +1,6 @@
 theory IsaSAT_Setup1_LLVM
   imports
+    IsaSAT_Setup
     IsaSAT_Setup0_LLVM
 begin
 
@@ -11,7 +12,7 @@ sepref_definition not_deleted_code
 
 lemma clause_not_marked_to_delete_heur_alt_def:
   \<open>RETURN oo clause_not_marked_to_delete_heur = (\<lambda> S C'. read_arena_wl_heur (\<lambda>N. do {status \<leftarrow> RETURN (arena_status N C'); RETURN (status \<noteq> DELETED)}) S)\<close>
-  by (auto intro!: ext simp: clause_not_marked_to_delete_heur_def read_all_wl_heur_def
+  by (auto intro!: ext simp: clause_not_marked_to_delete_heur_def read_all_st_def
     split: isasat_int.splits)
 
 definition clause_not_marked_to_delete_heur_code :: \<open>twl_st_wll_trail_fast2 \<Rightarrow> _ \<Rightarrow> _\<close> where
@@ -35,7 +36,7 @@ global_interpretation arena_is_valid: read_arena_param_adder where
 
 sepref_register clause_not_marked_to_delete_heur
 lemmas [sepref_fr_rules] = arena_is_valid.refine[unfolded uncurry_curry_id]
-lemmas [llvm_code] = clause_not_marked_to_delete_heur_code_def[unfolded read_all_wl_heur_code_def not_deleted_code_def]
+lemmas [llvm_code] = clause_not_marked_to_delete_heur_code_def[unfolded read_all_st_code_def not_deleted_code_def]
 
 
 sepref_def mop_clause_not_marked_to_delete_heur_impl
@@ -59,7 +60,7 @@ lemma conflict_is_None_code_refine[sepref_fr_rules]:
   done
 
 lemma get_conflict_wl_is_None_heur_alt_def: \<open>read_conflict_wl_heur conflict_is_None = RETURN \<circ> get_conflict_wl_is_None_heur\<close>
-  by (auto simp: read_all_wl_heur_def get_conflict_wl_is_None_heur_def conflict_is_None_def
+  by (auto simp: read_all_st_def get_conflict_wl_is_None_heur_def conflict_is_None_def
     intro!: ext split: isasat_int.splits)
 
 definition get_conflict_wl_is_None_heur2 where
@@ -84,17 +85,17 @@ global_interpretation conflict_is_None: read_conflict_param_adder0 where
 lemmas [sepref_fr_rules] = conflict_is_None.refine[unfolded get_conflict_wl_is_None_heur2_def]
 lemmas [llvm_code] = conflict_is_None_code_def
 lemmas [unfolded inline_direct_return_node_case, llvm_code] =
-  get_conflict_wl_is_None_fast_code_def[unfolded read_all_wl_heur_code_def]
+  get_conflict_wl_is_None_fast_code_def[unfolded read_all_st_code_def]
 
 lemma count_decided_st_heur_alt_def:
   \<open>RETURN o count_decided_st_heur = read_trail_wl_heur (RETURN \<circ> count_decided_pol)\<close>
   by (auto intro!: ext simp: count_decided_st_heur_def count_decided_pol_def
-    read_all_wl_heur_def split: isasat_int.splits)
+    read_all_st_def split: isasat_int.splits)
 
 definition count_decided_st_heur_impl where
   \<open>count_decided_st_heur_impl = read_trail_wl_heur_code count_decided_pol_impl\<close>
 
-sepref_register extract_trail_wl_heur count_decided_pol update_trail_wl_heur count_decided_st_heur
+sepref_register extract_trail_wl_heur count_decided_pol count_decided_st_heur
 
 
 definition isa_count_decided_st_fast_code :: \<open>twl_st_wll_trail_fast2 \<Rightarrow> _\<close> where
@@ -111,7 +112,7 @@ global_interpretation count_decided: read_trail_param_adder0 where
   apply unfold_locales
   apply (rule count_decided_pol_impl.refine)
   subgoal
-    by (auto simp: read_all_wl_heur_def isa_count_decided_st_def intro!: ext
+    by (auto simp: read_all_st_def isa_count_decided_st_def intro!: ext
       split: isasat_int.splits)
   subgoal
     by (auto simp: isa_count_decided_st_fast_code_def)
@@ -119,7 +120,7 @@ global_interpretation count_decided: read_trail_param_adder0 where
 
 lemmas [sepref_fr_rules] = count_decided.refine[unfolded lambda_comp_true]
 lemmas [unfolded inline_direct_return_node_case, llvm_code] =
-  isa_count_decided_st_fast_code_def[unfolded read_all_wl_heur_code_def]
+  isa_count_decided_st_fast_code_def[unfolded read_all_st_code_def]
 
 definition polarity_st_heur_pol_fast ::  \<open>twl_st_wll_trail_fast2 \<Rightarrow> _\<close>  where
   \<open>polarity_st_heur_pol_fast = (\<lambda>S C. read_trail_wl_heur_code (\<lambda>L. polarity_pol_fast L C) S)\<close>
@@ -138,13 +139,13 @@ global_interpretation mop_count_decided: read_trail_param_adder where
   subgoal
     by (auto simp: polarity_st_heur_pol_fast_def)
   subgoal
-    by (auto simp: mop_polarity_st_heur_def read_all_wl_heur_def
+    by (auto simp: mop_polarity_st_heur_def read_all_st_def
       split: isasat_int.splits intro!: ext)
   done
 
 lemmas [sepref_fr_rules] = mop_count_decided.refine[unfolded lambda_comp_true]
 lemmas [unfolded inline_direct_return_node_case, llvm_code] =
-  polarity_st_heur_pol_fast_def[unfolded read_all_wl_heur_code_def]
+  polarity_st_heur_pol_fast_def[unfolded read_all_st_code_def]
 
 definition arena_lit2 where \<open>arena_lit2 N i j = arena_lit N (i+j)\<close>
 
@@ -172,7 +173,7 @@ qed
 
 lemma access_lit_in_clauses_heur_alt_def:
   \<open>RETURN ooo access_lit_in_clauses_heur = (\<lambda>N C' D. read_arena_wl_heur (\<lambda>N. RETURN (arena_lit N (C' + D))) N)\<close>
-  by (auto intro!: ext simp: read_all_wl_heur_def access_lit_in_clauses_heur_def split: isasat_int.splits)
+  by (auto intro!: ext simp: read_all_st_def access_lit_in_clauses_heur_def split: isasat_int.splits)
 
 lemma access_lit_in_clauses_heur_pre:
   \<open>uncurry2
@@ -234,7 +235,7 @@ lemma refine_ASSERT_move_to_pre2':
 
 lemma arena_lit_arena_lit_read_arena_wl_heur_arena_lit:
   \<open>RETURN (arena_lit (get_clauses_wl_heur N) (C + C')) = read_arena_wl_heur (\<lambda>N. RETURN (arena_lit N (C + C'))) N\<close>
-  by (auto intro!: ext simp: read_all_wl_heur_def access_lit_in_clauses_heur_def split: isasat_int.splits)
+  by (auto intro!: ext simp: read_all_st_def access_lit_in_clauses_heur_def split: isasat_int.splits)
 
 sepref_register mop_access_lit_in_clauses_heur
 lemma mop_access_lit_in_clauses_heur_refine[sepref_fr_rules]:
@@ -266,7 +267,7 @@ sepref_def mop_access_lit_in_clauses_heur_impl
 lemmas [sepref_fr_rules] = access_arena.refine
 
 lemmas [unfolded inline_direct_return_node_case, llvm_code] =
-  access_lit_in_clauses_heur_fast_code_def[unfolded read_all_wl_heur_code_def]
+  access_lit_in_clauses_heur_fast_code_def[unfolded read_all_st_code_def]
 
 
 
@@ -304,17 +305,9 @@ lemma rewatch_heur_st_fast_alt_def:
   let S = update_vdom_wl_heur vdom S;
   RETURN S
   })\<close>
-  by (auto simp: rewatch_heur_st_fast_def rewatch_heur_st_def
-    extract_arena_wl_heur_def extract_watchlist_wl_heur_def extract_vdom_wl_heur_def
-    isasat_state_ops.remove_arena_wl_heur_def  isasat_state_ops.remove_watchlist_wl_heur_def  isasat_state_ops.remove_vdom_wl_heur_def
-    update_arena_wl_heur_def update_watchlist_wl_heur_def update_vdom_wl_heur_def
+  by (auto simp: rewatch_heur_st_fast_def rewatch_heur_st_def state_extractors
     split: isasat_int.splits
     intro!: ext)
-
-lemmas [sepref_fr_rules] =
-  remove_watchlist_wl_heur_code.refine
-  remove_vdom_wl_heur_code.refine
-  remove_arena_wl_heur_code.refine
 
 sepref_def rewatch_heur_st_fast_code
   is \<open>(rewatch_heur_st_fast)\<close>
@@ -336,7 +329,7 @@ global_interpretation length_ivdom_aivdom: read_vdom_param_adder0 where
   apply unfold_locales
   apply (rule vdom_ref)
   subgoal
-    by (auto simp: read_all_wl_heur_def length_ivdom_aivdom_def length_ivdom_def intro!: ext
+    by (auto simp: read_all_st_def length_ivdom_aivdom_def length_ivdom_def intro!: ext
       split: isasat_int.splits)
   subgoal
     by (auto simp: length_ivdom_fast_code_def)
@@ -355,7 +348,7 @@ global_interpretation length_avdom_aivdom: read_vdom_param_adder0 where
   apply unfold_locales
   apply (rule vdom_ref)
   subgoal
-    by (auto simp: read_all_wl_heur_def length_avdom_aivdom_def length_avdom_def intro!: ext
+    by (auto simp: read_all_st_def length_avdom_aivdom_def length_avdom_def intro!: ext
       split: isasat_int.splits)
   subgoal
     by (auto simp: length_avdom_fast_code_def)
@@ -375,7 +368,7 @@ global_interpretation length_tvdom_aivdom: read_vdom_param_adder0 where
   apply unfold_locales
   apply (rule vdom_ref)
   subgoal
-    by (auto simp: read_all_wl_heur_def length_tvdom_aivdom_def length_tvdom_def intro!: ext
+    by (auto simp: read_all_st_def length_tvdom_aivdom_def length_tvdom_def intro!: ext
       split: isasat_int.splits)
   subgoal
     by (auto simp: length_tvdom_fast_code_def)
@@ -387,9 +380,9 @@ lemmas [sepref_fr_rules] = length_ivdom_aivdom.refine[unfolded lambda_comp_true]
   length_tvdom_aivdom.refine[unfolded lambda_comp_true]
 
 lemmas [unfolded inline_direct_return_node_case, llvm_code] =
-  length_ivdom_fast_code_def[unfolded read_all_wl_heur_code_def]
-  length_avdom_fast_code_def[unfolded read_all_wl_heur_code_def]
-  length_tvdom_fast_code_def[unfolded read_all_wl_heur_code_def]
+  length_ivdom_fast_code_def[unfolded read_all_st_code_def]
+  length_avdom_fast_code_def[unfolded read_all_st_code_def]
+  length_tvdom_fast_code_def[unfolded read_all_st_code_def]
 
 sepref_register length_avdom length_ivdom length_tvdom
 
@@ -406,7 +399,7 @@ definition clause_is_learned_heur_code2 :: \<open>twl_st_wll_trail_fast2 \<Right
   \<open>clause_is_learned_heur_code2 N C = read_arena_wl_heur_code (\<lambda>Ca. is_learned_impl Ca C) N\<close>
 
 lemma clause_is_learned_heur_alt_def: \<open>RETURN oo clause_is_learned_heur = (\<lambda>N C'. read_arena_wl_heur (\<lambda>C. (RETURN \<circ>\<circ> is_learned) C C') N)\<close>
-  by (auto simp: clause_is_learned_heur_def read_all_wl_heur_def is_learned_def
+  by (auto simp: clause_is_learned_heur_def read_all_st_def is_learned_def
     intro!: ext split: isasat_int.splits)
 
 global_interpretation arena_is_learned: read_arena_param_adder where
@@ -431,7 +424,7 @@ definition clause_lbd_heur_code2 :: \<open>twl_st_wll_trail_fast2 \<Rightarrow> 
 
 lemma clause_lbd_heur_alt_def:
   \<open>RETURN \<circ>\<circ> clause_lbd_heur = (\<lambda>N C'. read_arena_wl_heur (\<lambda>C. (RETURN \<circ>\<circ> arena_lbd) C C') N)\<close>
-  by (auto simp: clause_lbd_heur_def read_all_wl_heur_def arena_lbd_def split: isasat_int.splits intro!: ext)
+  by (auto simp: clause_lbd_heur_def read_all_st_def arena_lbd_def split: isasat_int.splits intro!: ext)
 
 global_interpretation arena_get_lbd: read_arena_param_adder where
   R = \<open>(snat_rel' TYPE(64))\<close> and
@@ -448,7 +441,7 @@ global_interpretation arena_get_lbd: read_arena_param_adder where
   subgoal by (auto simp: clause_lbd_heur_code2_def intro!: ext)
   subgoal by (subst clause_lbd_heur_alt_def, rule refl)
   subgoal by (auto simp: mop_arena_lbd_st_def mop_arena_lbd_def read_arena_param_adder_ops.mop_def
-    read_all_wl_heur_def split: isasat_int.splits
+    read_all_st_def split: isasat_int.splits
     intro!: ext)
   done
 
@@ -471,16 +464,16 @@ global_interpretation arena_get_pos: read_arena_param_adder where
   apply (rule arena_pos_impl.refine)
   subgoal by (subst clause_pos_heur_code2_def, rule refl)
   subgoal by (auto simp: mop_arena_pos_st_def mop_arena_pos_def read_arena_param_adder_ops.mop_def
-    read_all_wl_heur_def split: isasat_int.splits
+    read_all_st_def split: isasat_int.splits
     intro!: ext)
   done
 
 lemmas [sepref_fr_rules] = arena_get_lbd.refine arena_get_pos.mop_refine
 
 lemmas [unfolded inline_direct_return_node_case, llvm_code] =
-  clause_lbd_heur_code2_def[unfolded read_all_wl_heur_code_def]
-  clause_is_learned_heur_code2_def[unfolded read_all_wl_heur_code_def]
-  clause_pos_heur_code2_def[unfolded read_all_wl_heur_code_def]
+  clause_lbd_heur_code2_def[unfolded read_all_st_code_def]
+  clause_is_learned_heur_code2_def[unfolded read_all_st_code_def]
+  clause_pos_heur_code2_def[unfolded read_all_st_code_def]
   is_learned_impl_def
 
 
@@ -578,8 +571,7 @@ lemma delete_index_vdom_heur_alt_def: \<open>RETURN oo delete_index_vdom_heur = 
   let vdom = remove_inactive_aivdom_tvdom i vdom;
   RETURN (update_vdom_wl_heur vdom S)
     })\<close>
-  by (auto simp: delete_index_vdom_heur_def extract_vdom_wl_heur_def
-    isasat_state_ops.remove_vdom_wl_heur_def update_vdom_wl_heur_def
+  by (auto simp: state_extractors delete_index_vdom_heur_def
     intro!: ext split: isasat_int.splits)
 
 sepref_def delete_index_vdom_heur_fast_code2
@@ -593,7 +585,7 @@ sepref_def delete_index_vdom_heur_fast_code2
 
 lemma access_length_heur_alt_def:
   \<open>RETURN oo access_length_heur = (\<lambda>N C'. read_arena_wl_heur (\<lambda>N. RETURN (arena_length N C')) N)\<close>
-  by (auto intro!: ext simp: read_all_wl_heur_def access_length_heur_def
+  by (auto intro!: ext simp: read_all_st_def access_length_heur_def
     split: isasat_int.splits)
 
 definition access_length_heur_fast_code2 :: \<open>twl_st_wll_trail_fast2 \<Rightarrow> _\<close> where
@@ -617,13 +609,13 @@ global_interpretation arena_length: read_arena_param_adder where
 lemmas [sepref_fr_rules] = arena_length.refine
 
 lemmas [unfolded inline_direct_return_node_case, llvm_code] =
-  access_length_heur_fast_code2_def[unfolded read_all_wl_heur_code_def]
+  access_length_heur_fast_code2_def[unfolded read_all_st_code_def]
 
 lemma get_slow_ema_heur_alt_def:
     \<open>RETURN o get_slow_ema_heur = read_heur_wl_heur (RETURN o slow_ema_of)\<close> and
   get_fast_ema_heur_alt_def:
     \<open>RETURN o get_fast_ema_heur = read_heur_wl_heur (RETURN o fast_ema_of)\<close> 
-  by (auto simp: read_all_wl_heur_def intro!: ext split: isasat_int.splits)
+  by (auto simp: read_all_st_def intro!: ext split: isasat_int.splits)
 
 definition get_slow_ema_heur_fast_code :: \<open>twl_st_wll_trail_fast2 \<Rightarrow> _\<close> where
   \<open>get_slow_ema_heur_fast_code = read_heur_wl_heur_code slow_ema_of_stats_impl\<close>
@@ -665,7 +657,7 @@ find_theorems get_conflict_count_since_last_restart RETURN
 lemma get_conflict_count_since_last_restart_heur_alt_def:
   \<open>RETURN o get_conflict_count_since_last_restart_heur =
   read_heur_wl_heur (RETURN \<circ> get_conflict_count_since_last_restart)\<close>
-  by (auto simp: read_all_wl_heur_def intro!: ext split: isasat_int.splits)
+  by (auto simp: read_all_st_def intro!: ext split: isasat_int.splits)
 
 definition get_conflict_count_since_last_restart_heur_fast_code :: \<open>twl_st_wll_trail_fast2 \<Rightarrow> _\<close> where
   \<open>get_conflict_count_since_last_restart_heur_fast_code = read_heur_wl_heur_code get_conflict_count_since_last_restart_stats_impl\<close>
@@ -690,7 +682,7 @@ lemma id_lcount_assn: \<open>(Mreturn, RETURN) \<in> (lcount_assn)\<^sup>k \<rig
   by sepref_to_hoare vcg
 
 lemma get_learned_count_alt_def: \<open>RETURN o get_learned_count = read_lcount_wl_heur RETURN\<close>
-  by (auto simp: read_all_wl_heur_def intro!: ext split: isasat_int.splits)
+  by (auto simp: read_all_st_def intro!: ext split: isasat_int.splits)
 
 definition get_learned_count_fast_code :: \<open>twl_st_wll_trail_fast2 \<Rightarrow> _\<close> where
   \<open>get_learned_count_fast_code = read_lcount_wl_heur_code Mreturn\<close>
@@ -722,7 +714,7 @@ global_interpretation get_learned_count_number: read_lcount_param_adder0 where
     \<open>read_lcount_wl_heur_code clss_size_lcount_fast_code = get_learned_count_number_fast_code\<close>
   apply unfold_locales
   apply (rule clss_size_lcount_fast_code.refine)
-  subgoal by (auto simp: read_all_wl_heur_def split: isasat_int.splits intro!: ext)
+  subgoal by (auto simp: read_all_st_def split: isasat_int.splits intro!: ext)
   subgoal by (auto simp: get_learned_count_number_fast_code_def)
   done
 
@@ -739,11 +731,11 @@ lemmas [sepref_fr_rules] =
   get_learned_count_number.refine[unfolded lambda_comp_true get_learned_count_number'_def[symmetric]]
   
 lemmas [unfolded inline_direct_return_node_case, llvm_code] =
-  get_slow_ema_heur_fast_code_def[unfolded read_all_wl_heur_code_def]
-  get_fast_ema_heur_fast_code_def[unfolded read_all_wl_heur_code_def]
-  get_conflict_count_since_last_restart_heur_fast_code_def[unfolded read_all_wl_heur_code_def]
-  get_learned_count_fast_code_def[unfolded read_all_wl_heur_code_def]
-  get_learned_count_number_fast_code_def[unfolded read_all_wl_heur_code_def]
+  get_slow_ema_heur_fast_code_def[unfolded read_all_st_code_def]
+  get_fast_ema_heur_fast_code_def[unfolded read_all_st_code_def]
+  get_conflict_count_since_last_restart_heur_fast_code_def[unfolded read_all_st_code_def]
+  get_learned_count_fast_code_def[unfolded read_all_st_code_def]
+  get_learned_count_number_fast_code_def[unfolded read_all_st_code_def]
 
 sepref_def learned_clss_count_fast_code
   is \<open>RETURN o learned_clss_count\<close>
@@ -764,18 +756,18 @@ global_interpretation marked_used: read_arena_param_adder where
   \<open>(\<lambda>N C. read_arena_wl_heur_code (\<lambda>N. marked_as_used_impl N C) N) = marked_as_used_st_fast_code\<close>
   apply unfold_locales
   apply (rule marked_as_used_impl.refine[unfolded comp_def])
-  subgoal by (auto simp: marked_as_used_st_def read_all_wl_heur_def intro!: ext split: isasat_int.splits)
+  subgoal by (auto simp: marked_as_used_st_def read_all_st_def intro!: ext split: isasat_int.splits)
   subgoal by (auto simp: marked_as_used_st_fast_code_def)
   done
 
 lemmas [sepref_fr_rules] = marked_used.refine
 
 lemmas [unfolded inline_direct_return_node_case, llvm_code] =
-  marked_as_used_st_fast_code_def[unfolded read_all_wl_heur_code_def]
+  marked_as_used_st_fast_code_def[unfolded read_all_st_code_def]
 
 lemma mop_marked_as_used_st_alt_def: \<open>mop_marked_as_used_st = marked_used.mop\<close>
   by (auto intro!: ext split: isasat_int.splits simp: mop_marked_as_used_st_def marked_used.mop_def
-    mop_marked_as_used_def read_all_wl_heur_def)
+    mop_marked_as_used_def read_all_st_def)
 
 lemmas [sepref_fr_rules] =
   marked_used.mop_refine[unfolded mop_marked_as_used_st_alt_def[symmetric]]
