Weidenbach_Book/IsaSAT/Tuple16_LLVM.thy
@@ -1,0 +1,1103 @@
+theory Tuple16_LLVM
+  imports Tuple16 IsaSAT_Literals_LLVM
+begin
+
+no_notation WB_More_Refinement.fref (\<open>[_]\<^sub>f _ \<rightarrow> _\<close> [0,60,60] 60)
+no_notation WB_More_Refinement.freft (\<open>_ \<rightarrow>\<^sub>f _\<close> [60,60] 60)
+hide_const (open) NEMonad.ASSERT NEMonad.RETURN
+
+
+instantiation isasat_int ::
+  (llvm_rep,llvm_rep,llvm_rep,llvm_rep,
+  llvm_rep,llvm_rep,llvm_rep,llvm_rep,
+  llvm_rep,llvm_rep,llvm_rep,llvm_rep,
+  llvm_rep,llvm_rep,llvm_rep,llvm_rep) llvm_rep
+begin
+  definition to_val_isasat_int where
+    \<open>to_val_isasat_int \<equiv> (\<lambda>S. case S of
+     IsaSAT_int M N D i W ivmtf icount ccach lbd outl stats heur aivdom clss opts arena \<Rightarrow> LL_STRUCT [to_val M, to_val N, to_val D, to_val i, to_val W, to_val ivmtf,
+       to_val icount, to_val ccach, to_val lbd,
+       to_val outl, to_val stats, to_val heur, to_val aivdom,  to_val clss, to_val opts, to_val arena])\<close>
+
+  definition from_val_isasat_int :: \<open>llvm_val \<Rightarrow> ('a, 'b, 'c, 'd, 'e, 'f, 'g, 'h, 'i, 'j, 'k, 'l, 'm, 'n, 'o, 'p) isasat_int\<close> where
+    \<open>from_val_isasat_int \<equiv> (\<lambda>p. case llvm_val.the_fields p of
+   [M, N, D, i, W, ivmtf, icount, ccach, lbd, outl, stats, heur, aivdom, clss, opts, arena] \<Rightarrow>
+     IsaSAT_int (from_val M) (from_val N) (from_val D) (from_val i) (from_val W) (from_val ivmtf) (from_val icount) (from_val ccach) (from_val lbd)
+       (from_val outl) (from_val stats) (from_val heur) (from_val aivdom) (from_val clss) (from_val opts) (from_val arena))\<close>
+
+  definition [simp]: "struct_of_isasat_int (_ :: ('a, 'b, 'c, 'd, 'e, 'f, 'g, 'h, 'i, 'j, 'k, 'l, 'm, 'n, 'o, 'p) isasat_int itself) \<equiv>
+     VS_STRUCT [struct_of TYPE('a), struct_of TYPE('b), struct_of TYPE('c),
+      struct_of TYPE('d), struct_of TYPE('e), struct_of TYPE('f), struct_of TYPE('g), struct_of TYPE('h),
+      struct_of TYPE('i), struct_of TYPE('j), struct_of TYPE('k), struct_of TYPE('l),
+      struct_of TYPE('m), struct_of TYPE('n), struct_of TYPE('o), struct_of TYPE('p)]"
+
+  definition [simp]: "init_isasat_int :: ('a, 'b, 'c, 'd, 'e, 'f, 'g, 'h, 'i, 'j, 'k, 'l, 'm, 'n, 'o, 'p) isasat_int \<equiv> IsaSAT_int init init init init init init init init init init init init init init init init"
+
+  instance
+    apply standard
+    unfolding from_val_isasat_int_def to_val_isasat_int_def struct_of_isasat_int_def init_isasat_int_def comp_def isasat_int.case_distrib
+    subgoal
+      by (auto simp: init_zero fun_eq_iff from_val_isasat_int_def split: isasat_int.splits)
+    subgoal for v
+      by (cases v) (auto split: list.splits isasat_int.splits)
+    subgoal for v
+      by (cases v)
+       (simp add: LLVM_Shallow.null_def to_val_ptr_def split: isasat_int.splits)
+    subgoal
+      by (simp add: LLVM_Shallow.null_def to_val_ptr_def to_val_word_def init_zero split: isasat_int.splits)
+    done
+end
+
+subsubsection \<open>Setup for LLVM code export\<close>
+text \<open>Declare structure to code generator.\<close>
+lemma to_val_isasat_int[ll_to_val]: "to_val x = LL_STRUCT [
+  to_val (Tuple16_get_a x),
+  to_val (Tuple16_get_b x),
+  to_val (Tuple16_get_c x),
+  to_val (Tuple16_get_d x),
+  to_val (Tuple16_get_e x),
+  to_val (Tuple16_get_f x),
+  to_val (Tuple16_get_g x),
+  to_val (Tuple16_get_h x),
+  to_val (Tuple16_get_i x),
+  to_val (Tuple16_get_j x),
+  to_val (Tuple16_get_k x),
+  to_val (Tuple16_get_l x),
+  to_val (Tuple16_get_m x),
+  to_val (Tuple16_get_n x),
+  to_val (Tuple16_get_o x),
+  to_val (Tuple16_get_p x)]"
+  apply (cases x)
+  apply (auto simp: to_val_isasat_int_def)
+  done
+
+lemma node_insert_value:
+  "ll_insert_value (IsaSAT_int M N D i W ivmtf icount ccach lbd outl stats heur aivdom clss opts arena) M' 0 = Mreturn (IsaSAT_int M' N D i W ivmtf icount ccach lbd outl stats heur aivdom clss opts arena)"
+  "ll_insert_value (IsaSAT_int M N D i W ivmtf icount ccach lbd outl stats heur aivdom clss opts arena) N' (Suc 0) = Mreturn (IsaSAT_int M N' D i W ivmtf icount ccach lbd outl stats heur aivdom clss opts arena)"
+  "ll_insert_value (IsaSAT_int M N D i W ivmtf icount ccach lbd outl stats heur aivdom clss opts arena) D' 2 = Mreturn (IsaSAT_int M N D' i W ivmtf icount ccach lbd outl stats heur aivdom clss opts arena)"
+  "ll_insert_value (IsaSAT_int M N D i W ivmtf icount ccach lbd outl stats heur aivdom clss opts arena) i' 3 = Mreturn (IsaSAT_int M N D i' W ivmtf icount ccach lbd outl stats heur aivdom clss opts arena)"
+  "ll_insert_value (IsaSAT_int M N D i W ivmtf icount ccach lbd outl stats heur aivdom clss opts arena) W' 4 = Mreturn (IsaSAT_int M N D i W' ivmtf icount ccach lbd outl stats heur aivdom clss opts arena)"
+  "ll_insert_value (IsaSAT_int M N D i W ivmtf icount ccach lbd outl stats heur aivdom clss opts arena) ivmtf' 5 = Mreturn (IsaSAT_int M N D i W ivmtf' icount ccach lbd outl stats heur aivdom clss opts arena)"
+  "ll_insert_value (IsaSAT_int M N D i W ivmtf icount ccach lbd outl stats heur aivdom clss opts arena) icount' 6 = Mreturn (IsaSAT_int M N D i W ivmtf icount' ccach lbd outl stats heur aivdom clss opts arena)"
+  "ll_insert_value (IsaSAT_int M N D i W ivmtf icount ccach lbd outl stats heur aivdom clss opts arena) ccach' 7 = Mreturn (IsaSAT_int M N D i W ivmtf icount ccach' lbd outl stats heur aivdom clss opts arena)"
+  "ll_insert_value (IsaSAT_int M N D i W ivmtf icount ccach lbd outl stats heur aivdom clss opts arena) lbd' 8 = Mreturn (IsaSAT_int M N D i W ivmtf icount ccach lbd' outl stats heur aivdom clss opts arena)"
+  "ll_insert_value (IsaSAT_int M N D i W ivmtf icount ccach lbd outl stats heur aivdom clss opts arena) outl' 9 = Mreturn (IsaSAT_int M N D i W ivmtf icount ccach lbd outl' stats heur aivdom clss opts arena)"
+  "ll_insert_value (IsaSAT_int M N D i W ivmtf icount ccach lbd outl stats heur aivdom clss opts arena) stats' 10 = Mreturn (IsaSAT_int M N D i W ivmtf icount ccach lbd outl stats' heur aivdom clss opts arena)"
+  "ll_insert_value (IsaSAT_int M N D i W ivmtf icount ccach lbd outl stats heur aivdom clss opts arena) heur' 11 = Mreturn (IsaSAT_int M N D i W ivmtf icount ccach lbd outl stats heur' aivdom clss opts arena)"
+  "ll_insert_value (IsaSAT_int M N D i W ivmtf icount ccach lbd outl stats heur aivdom clss opts arena) aivdom' 12 = Mreturn (IsaSAT_int M N D i W ivmtf icount ccach lbd outl stats heur aivdom' clss opts arena)"
+  "ll_insert_value (IsaSAT_int M N D i W ivmtf icount ccach lbd outl stats heur aivdom clss opts arena) clss' 13 = Mreturn (IsaSAT_int M N D i W ivmtf icount ccach lbd outl stats heur aivdom clss' opts arena)"
+  "ll_insert_value (IsaSAT_int M N D i W ivmtf icount ccach lbd outl stats heur aivdom clss opts arena) opts' 14 = Mreturn (IsaSAT_int M N D i W ivmtf icount ccach lbd outl stats heur aivdom clss opts' arena)"
+  "ll_insert_value (IsaSAT_int M N D i W ivmtf icount ccach lbd outl stats heur aivdom clss opts arena) arena' 15 = Mreturn (IsaSAT_int M N D i W ivmtf icount ccach lbd outl stats heur aivdom clss opts arena')"
+  by (simp_all add: ll_insert_value_def llvm_insert_value_def Let_def checked_from_val_def
+                to_val_isasat_int_def from_val_isasat_int_def)
+
+lemma node_extract_value:
+  "ll_extract_value (IsaSAT_int M N D i W ivmtf icount ccach lbd outl stats heur aivdom clss opts arena) 0 = Mreturn M"
+  "ll_extract_value (IsaSAT_int M N D i W ivmtf icount ccach lbd outl stats heur aivdom clss opts arena) (Suc 0) = Mreturn N"
+  "ll_extract_value (IsaSAT_int M N D i W ivmtf icount ccach lbd outl stats heur aivdom clss opts arena) 2 = Mreturn D"
+  "ll_extract_value (IsaSAT_int M N D i W ivmtf icount ccach lbd outl stats heur aivdom clss opts arena) 3 = Mreturn i"
+  "ll_extract_value (IsaSAT_int M N D i W ivmtf icount ccach lbd outl stats heur aivdom clss opts arena) 4 = Mreturn W"
+  "ll_extract_value (IsaSAT_int M N D i W ivmtf icount ccach lbd outl stats heur aivdom clss opts arena) 5 = Mreturn ivmtf"
+  "ll_extract_value (IsaSAT_int M N D i W ivmtf icount ccach lbd outl stats heur aivdom clss opts arena) 6 = Mreturn icount"
+  "ll_extract_value (IsaSAT_int M N D i W ivmtf icount ccach lbd outl stats heur aivdom clss opts arena) 7 = Mreturn ccach"
+  "ll_extract_value (IsaSAT_int M N D i W ivmtf icount ccach lbd outl stats heur aivdom clss opts arena) 8 = Mreturn lbd"
+  "ll_extract_value (IsaSAT_int M N D i W ivmtf icount ccach lbd outl stats heur aivdom clss opts arena) 9 = Mreturn outl"
+  "ll_extract_value (IsaSAT_int M N D i W ivmtf icount ccach lbd outl stats heur aivdom clss opts arena) 10 = Mreturn stats"
+  "ll_extract_value (IsaSAT_int M N D i W ivmtf icount ccach lbd outl stats heur aivdom clss opts arena) 11 = Mreturn heur"
+  "ll_extract_value (IsaSAT_int M N D i W ivmtf icount ccach lbd outl stats heur aivdom clss opts arena) 12 = Mreturn aivdom"
+  "ll_extract_value (IsaSAT_int M N D i W ivmtf icount ccach lbd outl stats heur aivdom clss opts arena) 13 = Mreturn clss"
+  "ll_extract_value (IsaSAT_int M N D i W ivmtf icount ccach lbd outl stats heur aivdom clss opts arena) 14 = Mreturn opts"
+  "ll_extract_value (IsaSAT_int M N D i W ivmtf icount ccach lbd outl stats heur aivdom clss opts arena) 15 = Mreturn arena"
+  apply (simp_all add: ll_extract_value_def llvm_extract_value_def Let_def checked_from_val_def
+                to_val_isasat_int_def from_val_isasat_int_def)
+  done
+
+text \<open>Lemmas to translate node construction and destruction\<close>
+lemma inline_return_node[llvm_pre_simp]: "Mreturn (IsaSAT_int M N D i W ivmtf icount ccach lbd outl heur stats aivdom clss opts arena) = doM {
+    r \<leftarrow> ll_insert_value init M 0;
+    r \<leftarrow> ll_insert_value r N 1;
+    r \<leftarrow> ll_insert_value r D 2;
+    r \<leftarrow> ll_insert_value r i 3;
+    r \<leftarrow> ll_insert_value r W 4;
+    r \<leftarrow> ll_insert_value r ivmtf 5;
+    r \<leftarrow> ll_insert_value r icount 6;
+    r \<leftarrow> ll_insert_value r ccach 7;
+    r \<leftarrow> ll_insert_value r lbd 8;
+    r \<leftarrow> ll_insert_value r outl 9;
+    r \<leftarrow> ll_insert_value r heur 10;
+    r \<leftarrow> ll_insert_value r stats 11;
+    r \<leftarrow> ll_insert_value r aivdom 12;
+    r \<leftarrow> ll_insert_value r clss 13;
+    r \<leftarrow> ll_insert_value r opts 14;
+    r \<leftarrow> ll_insert_value r arena 15;
+    Mreturn r
+  }"
+  apply (auto simp: node_insert_value)
+  done
+
+lemma inline_node_case[llvm_pre_simp]: "(case r of (IsaSAT_int M N D i W ivmtf icount ccach lbd outl heur stats aivdom clss opts arena) \<Rightarrow> f M N D i W ivmtf icount ccach lbd outl heur stats aivdom clss opts arena) = doM {
+    M \<leftarrow> ll_extract_value r 0;
+    N \<leftarrow> ll_extract_value r 1;
+    D \<leftarrow> ll_extract_value r 2;
+    i \<leftarrow> ll_extract_value r 3;
+    W \<leftarrow> ll_extract_value r 4;
+    ivmtf \<leftarrow> ll_extract_value r 5;
+    icount \<leftarrow> ll_extract_value r 6;
+    ccach \<leftarrow> ll_extract_value r 7;
+    lbd \<leftarrow> ll_extract_value r 8;
+    outl \<leftarrow> ll_extract_value r 9;
+    heur \<leftarrow> ll_extract_value r 10;
+    stats \<leftarrow> ll_extract_value r 11;
+    aivdom \<leftarrow> ll_extract_value r 12;
+    clss \<leftarrow> ll_extract_value r 13;
+    opts \<leftarrow> ll_extract_value r 14;
+    arena \<leftarrow> ll_extract_value r 15;
+  f M N D i W ivmtf icount ccach lbd outl heur stats aivdom clss opts arena
+}"
+  apply (cases r)
+  apply (auto simp: node_extract_value)
+  done
+
+lemma inline_return_node_case[llvm_pre_simp]: "doM {Mreturn (case r of (IsaSAT_int M N D i W ivmtf icount ccach lbd outl heur stats aivdom clss opts arena) \<Rightarrow> f M N D i W ivmtf icount ccach lbd outl heur stats aivdom clss opts arena)} = doM {
+    M \<leftarrow> ll_extract_value r 0;
+    N \<leftarrow> ll_extract_value r 1;
+    D \<leftarrow> ll_extract_value r 2;
+    i \<leftarrow> ll_extract_value r 3;
+    W \<leftarrow> ll_extract_value r 4;
+    ivmtf \<leftarrow> ll_extract_value r 5;
+    icount \<leftarrow> ll_extract_value r 6;
+    ccach \<leftarrow> ll_extract_value r 7;
+    lbd \<leftarrow> ll_extract_value r 8;
+    outl \<leftarrow> ll_extract_value r 9;
+    heur \<leftarrow> ll_extract_value r 10;
+    stats \<leftarrow> ll_extract_value r 11;
+    aivdom \<leftarrow> ll_extract_value r 12;
+    clss \<leftarrow> ll_extract_value r 13;
+    opts \<leftarrow> ll_extract_value r 14;
+    arena \<leftarrow> ll_extract_value r 15;
+  Mreturn (f M N D i W ivmtf icount ccach lbd outl heur stats aivdom clss opts arena)
+}"
+  apply (cases r)
+  apply (auto simp: node_extract_value)
+  done
+lemma inline_direct_return_node_case[llvm_pre_simp]: "doM {(case r of (IsaSAT_int M N D i W ivmtf icount ccach lbd outl heur stats aivdom clss opts arena) \<Rightarrow> f M N D i W ivmtf icount ccach lbd outl heur stats aivdom clss opts arena)} = doM {
+    M \<leftarrow> ll_extract_value r 0;
+    N \<leftarrow> ll_extract_value r 1;
+    D \<leftarrow> ll_extract_value r 2;
+    i \<leftarrow> ll_extract_value r 3;
+    W \<leftarrow> ll_extract_value r 4;
+    ivmtf \<leftarrow> ll_extract_value r 5;
+    icount \<leftarrow> ll_extract_value r 6;
+    ccach \<leftarrow> ll_extract_value r 7;
+    lbd \<leftarrow> ll_extract_value r 8;
+    outl \<leftarrow> ll_extract_value r 9;
+    heur \<leftarrow> ll_extract_value r 10;
+    stats \<leftarrow> ll_extract_value r 11;
+    aivdom \<leftarrow> ll_extract_value r 12;
+    clss \<leftarrow> ll_extract_value r 13;
+    opts \<leftarrow> ll_extract_value r 14;
+    arena \<leftarrow> ll_extract_value r 15;
+   (f M N D i W ivmtf icount ccach lbd outl heur stats aivdom clss opts arena)
+}"
+  apply (cases r)
+  apply (auto simp: node_extract_value)
+  done
+
+lemmas [llvm_inline] =
+  isasat_int.Tuple16_get_a_def
+  isasat_int.Tuple16_get_b_def
+  isasat_int.Tuple16_get_c_def
+  isasat_int.Tuple16_get_d_def
+  isasat_int.Tuple16_get_e_def
+  isasat_int.Tuple16_get_f_def
+  isasat_int.Tuple16_get_g_def
+  isasat_int.Tuple16_get_h_def
+  isasat_int.Tuple16_get_i_def
+  isasat_int.Tuple16_get_j_def
+  isasat_int.Tuple16_get_l_def
+  isasat_int.Tuple16_get_k_def
+  isasat_int.Tuple16_get_m_def
+  isasat_int.Tuple16_get_n_def
+  isasat_int.Tuple16_get_o_def
+  isasat_int.Tuple16_get_p_def
+
+fun isasat_int_assn :: \<open>
+  ('a \<Rightarrow> _ \<Rightarrow> llvm_amemory \<Rightarrow> bool) \<Rightarrow>
+  ('b \<Rightarrow> _ \<Rightarrow> llvm_amemory \<Rightarrow> bool) \<Rightarrow>
+  ('c \<Rightarrow> _ \<Rightarrow> llvm_amemory \<Rightarrow> bool) \<Rightarrow>
+  ('d \<Rightarrow> _ \<Rightarrow> llvm_amemory \<Rightarrow> bool) \<Rightarrow>
+  ('e \<Rightarrow> _ \<Rightarrow> llvm_amemory \<Rightarrow> bool) \<Rightarrow>
+  ('f \<Rightarrow> _ \<Rightarrow> llvm_amemory \<Rightarrow> bool) \<Rightarrow>
+  ('g \<Rightarrow> _ \<Rightarrow> llvm_amemory \<Rightarrow> bool) \<Rightarrow>
+  ('h \<Rightarrow> _ \<Rightarrow> llvm_amemory \<Rightarrow> bool) \<Rightarrow>
+  ('i \<Rightarrow> _ \<Rightarrow> llvm_amemory \<Rightarrow> bool) \<Rightarrow>
+  ('j \<Rightarrow> _ \<Rightarrow> llvm_amemory \<Rightarrow> bool) \<Rightarrow>
+  ('k \<Rightarrow> _ \<Rightarrow> llvm_amemory \<Rightarrow> bool) \<Rightarrow>
+  ('l \<Rightarrow> _ \<Rightarrow> llvm_amemory \<Rightarrow> bool) \<Rightarrow>
+  ('m \<Rightarrow> _ \<Rightarrow> llvm_amemory \<Rightarrow> bool) \<Rightarrow>
+  ('n \<Rightarrow> _ \<Rightarrow> llvm_amemory \<Rightarrow> bool) \<Rightarrow>
+  ('o \<Rightarrow> _ \<Rightarrow> llvm_amemory \<Rightarrow> bool) \<Rightarrow>
+  ('p \<Rightarrow> _ \<Rightarrow> llvm_amemory \<Rightarrow> bool) \<Rightarrow>
+  ('a, 'b, 'c, 'd, 'e, 'f, 'g, 'h, 'i, 'j,
+     'k, 'l, 'm, 'n, 'o, 'p) isasat_int \<Rightarrow> _ \<Rightarrow> assn\<close> where
+  \<open>isasat_int_assn a_assn b_assn' c_assn d_assn e_assn f_assn g_assn h_assn i_assn j_assn k_assn l_assn m_assn n_assn o_assn p_assn S T =
+   (case (S, T) of
+  (IsaSAT_int M N D i W ivmtf icount ccach lbd outl heur stats aivdom clss opts arena,
+   IsaSAT_int M' N' D' i' W' ivmtf' icount' ccach' lbd' outl' heur' stats' aivdom' clss' opts' arena')
+     \<Rightarrow>
+ (a_assn M (M') \<and>* b_assn' N (N') \<and>* c_assn D (D')  \<and>* d_assn i (i') \<and>*
+ e_assn W (W') \<and>* f_assn ivmtf (ivmtf') \<and>* g_assn icount (icount')  \<and>* h_assn ccach (ccach') \<and>*
+ i_assn lbd (lbd') \<and>* j_assn outl (outl') \<and>* k_assn heur (heur')  \<and>* l_assn stats (stats') \<and>*
+ m_assn aivdom (aivdom') \<and>* n_assn clss (clss') \<and>* o_assn opts (opts')  \<and>* p_assn arena (arena')))
+  \<close>
+
+
+locale isasat_state_ops =
+  fixes
+    a_assn :: \<open>'a \<Rightarrow> 'xa \<Rightarrow> assn\<close> and
+    b_assn :: \<open>'b \<Rightarrow> 'xb \<Rightarrow> assn\<close> and
+    c_assn :: \<open>'c \<Rightarrow> 'xc \<Rightarrow> assn\<close> and
+    d_assn :: \<open>'d \<Rightarrow> 'xd \<Rightarrow> assn\<close> and
+    e_assn :: \<open>'e \<Rightarrow> 'xe \<Rightarrow> assn\<close> and
+    f_assn :: \<open>'f \<Rightarrow> 'xf \<Rightarrow> assn\<close> and
+    g_assn :: \<open>'g \<Rightarrow> 'xg \<Rightarrow> assn\<close> and
+    h_assn :: \<open>'h \<Rightarrow> 'xh \<Rightarrow> assn\<close> and
+    i_assn :: \<open>'i \<Rightarrow> 'xi \<Rightarrow> assn\<close> and
+    j_assn :: \<open>'j \<Rightarrow> 'xj \<Rightarrow> assn\<close> and
+    k_assn :: \<open>'k \<Rightarrow> 'xk \<Rightarrow> assn\<close> and
+    l_assn :: \<open>'l \<Rightarrow> 'xl \<Rightarrow> assn\<close> and
+    m_assn :: \<open>'m \<Rightarrow> 'xm \<Rightarrow> assn\<close> and
+    n_assn :: \<open>'n \<Rightarrow> 'xn \<Rightarrow> assn\<close> and
+    o_assn :: \<open>'o \<Rightarrow> 'xo \<Rightarrow> assn\<close> and
+    p_assn :: \<open>'p \<Rightarrow> 'xp \<Rightarrow> assn\<close> and
+    a_default :: 'a and
+    a :: \<open>'xa llM\<close> and
+    b_default :: 'b and
+    b :: \<open>'xb llM\<close> and
+    c_default :: 'c and
+    c :: \<open>'xc llM\<close> and
+    d_default :: 'd and
+    d :: \<open>'xd llM\<close> and
+    e_default :: 'e and
+    e :: \<open>'xe llM\<close> and
+    f_default :: 'f and
+    f :: \<open>'xf llM\<close> and
+    g_default :: 'g and
+    g :: \<open>'xg llM\<close> and
+    h_default :: 'h and
+    h :: \<open>'xh llM\<close> and
+    i_default :: 'i and
+    i :: \<open>'xi llM\<close> and
+    j_default :: 'j and
+    j :: \<open>'xj llM\<close> and
+    k_default :: 'k and
+    k :: \<open>'xk llM\<close> and
+    l_default :: 'l and
+    l :: \<open>'xl llM\<close> and
+    m_default :: 'm and
+    m :: \<open>'xm llM\<close> and
+    n_default :: 'n and
+    n :: \<open>'xn llM\<close> and
+    ko_default :: 'o and
+    ko :: \<open>'xo llM\<close> and
+    p_default :: 'p and
+    p :: \<open>'xp llM\<close>
+begin
+
+definition isasat_assn :: \<open>_ \<Rightarrow> _ \<Rightarrow> assn\<close> where
+\<open>isasat_assn = isasat_int_assn
+  a_assn b_assn c_assn d_assn
+  e_assn f_assn g_assn h_assn
+  i_assn j_assn k_assn l_assn
+  m_assn n_assn o_assn p_assn\<close>
+
+definition remove_a :: \<open>('a, 'b, 'c, 'd, 'e, 'f, 'g, 'h, 'i, 'j,
+     'k, 'l, 'm, 'n, 'o, 'p) isasat_int \<Rightarrow> _ \<times> ('a, 'b, 'c, 'd, 'e, 'f, 'g, 'h, 'i, 'j,
+     'k, 'l, 'm, 'n, 'o, 'p) isasat_int\<close> where
+  \<open>remove_a isasat_int = (case isasat_int of IsaSAT_int x1 x2 x3 x4 x5 x6 x7 x8 x9 x10 x11 x12 x13 x14 x15 x16 \<Rightarrow>
+      (x1, IsaSAT_int a_default x2 x3 x4 x5 x6 x7 x8 x9 x10 x11 x12 x13 x14 x15 x16))\<close>
+
+definition remove_b :: \<open>('a, 'b, 'c, 'd, 'e, 'f, 'g, 'h, 'i, 'j,
+     'k, 'l, 'm, 'n, 'o, 'p) isasat_int \<Rightarrow> 'b \<times> ('a, 'b, 'c, 'd, 'e, 'f, 'g, 'h, 'i, 'j,
+     'k, 'l, 'm, 'n, 'o, 'p) isasat_int\<close> where
+  \<open>remove_b isasat_int = (case isasat_int of IsaSAT_int x1 x2 x3 x4 x5 x6 x7 x8 x9 x10 x11 x12 x13 x14 x15 x16 \<Rightarrow>
+      (x2, IsaSAT_int x1 b_default x3 x4 x5 x6 x7 x8 x9 x10 x11 x12 x13 x14 x15 x16))\<close>
+
+definition remove_c:: \<open>('a, 'b, 'c, 'd, 'e, 'f, 'g, 'h, 'i, 'j,
+     'k, 'l, 'm, 'n, 'o, 'p) isasat_int \<Rightarrow> _ \<times> ('a, 'b, 'c, 'd, 'e, 'f, 'g, 'h, 'i, 'j,
+     'k, 'l, 'm, 'n, 'o, 'p) isasat_int\<close> where
+  \<open>remove_c isasat_int = (case isasat_int of IsaSAT_int x1 x2 x3 x4 x5 x6 x7 x8 x9 x10 x11 x12 x13 x14 x15 x16 \<Rightarrow>
+      (x3, IsaSAT_int x1 x2 c_default x4 x5 x6 x7 x8 x9 x10 x11 x12 x13 x14 x15 x16))\<close>
+
+definition remove_d :: \<open>('a, 'b, 'c, 'd, 'e, 'f, 'g, 'h, 'i, 'j,
+     'k, 'l, 'm, 'n, 'o, 'p) isasat_int \<Rightarrow> _ \<times> ('a, 'b, 'c, 'd, 'e, 'f, 'g, 'h, 'i, 'j,
+     'k, 'l, 'm, 'n, 'o, 'p) isasat_int\<close> where
+  \<open>remove_d isasat_int = (case isasat_int of IsaSAT_int x1 x2 x3 x4 x5 x6 x7 x8 x9 x10 x11 x12 x13 x14 x15 x16 \<Rightarrow>
+      (x4, IsaSAT_int x1 x2 x3 d_default x5 x6 x7 x8 x9 x10 x11 x12 x13 x14 x15 x16))\<close>
+
+definition remove_e :: \<open>('a, 'b, 'c, 'd, 'e, 'f, 'g, 'h, 'i, 'j,
+     'k, 'l, 'm, 'n, 'o, 'p) isasat_int \<Rightarrow> 'e \<times> ('a, 'b, 'c, 'd, 'e, 'f, 'g, 'h, 'i, 'j,
+     'k, 'l, 'm, 'n, 'o, 'p) isasat_int\<close> where
+  \<open>remove_e isasat_int = (case isasat_int of IsaSAT_int x1 x2 x3 x4 x5 x6 x7 x8 x9 x10 x11 x12 x13 x14 x15 x16 \<Rightarrow>
+      (x5, IsaSAT_int x1 x2 x3 x4 e_default x6 x7 x8 x9 x10 x11 x12 x13 x14 x15 x16))\<close>
+
+definition remove_f :: \<open>('a, 'b, 'c, 'd, 'e, 'f, 'g, 'h, 'i, 'j,
+     'k, 'l, 'm, 'n, 'o, 'p) isasat_int \<Rightarrow> 'f \<times> ('a, 'b, 'c, 'd, 'e, 'f, 'g, 'h, 'i, 'j,
+     'k, 'l, 'm, 'n, 'o, 'p) isasat_int\<close> where
+  \<open>remove_f isasat_int = (case isasat_int of IsaSAT_int x1 x2 x3 x4 x5 x6 x7 x8 x9 x10 x11 x12 x13 x14 x15 x16 \<Rightarrow>
+      (x6, IsaSAT_int x1 x2 x3 x4 x5 f_default x7 x8 x9 x10 x11 x12 x13 x14 x15 x16))\<close>
+
+definition remove_g :: \<open>('a, 'b, 'c, 'd, 'e, 'f, 'g, 'h, 'i, 'j,
+     'k, 'l, 'm, 'n, 'o, 'p) isasat_int \<Rightarrow> 'g \<times> ('a, 'b, 'c, 'd, 'e, 'f, 'g, 'h, 'i, 'j,
+     'k, 'l, 'm, 'n, 'o, 'p) isasat_int\<close> where
+  \<open>remove_g isasat_int = (case isasat_int of IsaSAT_int x1 x2 x3 x4 x5 x6 x7 x8 x9 x10 x11 x12 x13 x14 x15 x16 \<Rightarrow>
+      (x7, IsaSAT_int x1 x2 x3 x4 x5 x6 g_default x8 x9 x10 x11 x12 x13 x14 x15 x16))\<close>
+
+definition remove_h :: \<open>('a, 'b, 'c, 'd, 'e, 'f, 'g, 'h, 'i, 'j,
+     'k, 'l, 'm, 'n, 'o, 'p) isasat_int \<Rightarrow> 'h \<times> ('a, 'b, 'c, 'd, 'e, 'f, 'g, 'h, 'i, 'j,
+     'k, 'l, 'm, 'n, 'o, 'p) isasat_int\<close> where
+  \<open>remove_h isasat_int = (case isasat_int of IsaSAT_int x1 x2 x3 x4 x5 x6 x7 x8 x9 x10 x11 x12 x13 x14 x15 x16 \<Rightarrow>
+      (x8, IsaSAT_int x1 x2 x3 x4 x5 x6 x7 h_default x9 x10 x11 x12 x13 x14 x15 x16))\<close>
+
+definition remove_i :: \<open>('a, 'b, 'c, 'd, 'e, 'f, 'g, 'h, 'i, 'j,
+     'k, 'l, 'm, 'n, 'o, 'p) isasat_int \<Rightarrow> 'i \<times> ('a, 'b, 'c, 'd, 'e, 'f, 'g, 'h, 'i, 'j,
+     'k, 'l, 'm, 'n, 'o, 'p) isasat_int\<close> where
+  \<open>remove_i isasat_int = (case isasat_int of IsaSAT_int x1 x2 x3 x4 x5 x6 x7 x8 x9 x10 x11 x12 x13 x14 x15 x16 \<Rightarrow>
+      (x9, IsaSAT_int x1 x2 x3 x4 x5 x6 x7 x8 i_default x10 x11 x12 x13 x14 x15 x16))\<close>
+
+definition remove_j :: \<open>('a, 'b, 'c, 'd, 'e, 'f, 'g, 'h, 'i, 'j,
+     'k, 'l, 'm, 'n, 'o, 'p) isasat_int \<Rightarrow> 'j \<times> ('a, 'b, 'c, 'd, 'e, 'f, 'g, 'h, 'i, 'j,
+     'k, 'l, 'm, 'n, 'o, 'p) isasat_int\<close> where
+  \<open>remove_j isasat_int = (case isasat_int of IsaSAT_int x1 x2 x3 x4 x5 x6 x7 x8 x9 x10 x11 x12 x13 x14 x15 x16 \<Rightarrow>
+      (x10, IsaSAT_int x1 x2 x3 x4 x5 x6 x7 x8 x9 j_default x11 x12 x13 x14 x15 x16))\<close>
+
+definition remove_k :: \<open>('a, 'b, 'c, 'd, 'e, 'f, 'g, 'h, 'i, 'j,
+     'k, 'l, 'm, 'n, 'o, 'p) isasat_int \<Rightarrow> 'k \<times> ('a, 'b, 'c, 'd, 'e, 'f, 'g, 'h, 'i, 'j,
+     'k, 'l, 'm, 'n, 'o, 'p) isasat_int\<close> where
+  \<open>remove_k isasat_int = (case isasat_int of IsaSAT_int x1 x2 x3 x4 x5 x6 x7 x8 x9 x10 x11 x12 x13 x14 x15 x16 \<Rightarrow>
+      (x11, IsaSAT_int x1 x2 x3 x4 x5 x6 x7 x8 x9 x10 k_default x12 x13 x14 x15 x16))\<close>
+
+definition remove_l :: \<open>('a, 'b, 'c, 'd, 'e, 'f, 'g, 'h, 'i, 'j,
+     'k, 'l, 'm, 'n, 'o, 'p) isasat_int \<Rightarrow> 'l \<times> ('a, 'b, 'c, 'd, 'e, 'f, 'g, 'h, 'i, 'j,
+     'k, 'l, 'm, 'n, 'o, 'p) isasat_int\<close> where
+  \<open>remove_l isasat_int = (case isasat_int of IsaSAT_int x1 x2 x3 x4 x5 x6 x7 x8 x9 x10 x11 x12 x13 x14 x15 x16 \<Rightarrow>
+      (x12, IsaSAT_int x1 x2 x3 x4 x5 x6 x7 x8 x9 x10 x11 l_default x13 x14 x15 x16))\<close>
+
+definition remove_m :: \<open>('a, 'b, 'c, 'd, 'e, 'f, 'g, 'h, 'i, 'j,
+     'k, 'l, 'm, 'n, 'o, 'p) isasat_int \<Rightarrow> 'm \<times> ('a, 'b, 'c, 'd, 'e, 'f, 'g, 'h, 'i, 'j,
+     'k, 'l, 'm, 'n, 'o, 'p) isasat_int\<close> where
+  \<open>remove_m isasat_int = (case isasat_int of IsaSAT_int x1 x2 x3 x4 x5 x6 x7 x8 x9 x10 x11 x12 x13 x14 x15 x16 \<Rightarrow>
+      (x13, IsaSAT_int x1 x2 x3 x4 x5 x6 x7 x8 x9 x10 x11 x12 m_default x14 x15 x16))\<close>
+
+definition remove_n :: \<open>('a, 'b, 'c, 'd, 'e, 'f, 'g, 'h, 'i, 'j,
+     'k, 'l, 'm, 'n, 'o, 'p) isasat_int \<Rightarrow> 'n \<times> ('a, 'b, 'c, 'd, 'e, 'f, 'g, 'h, 'i, 'j,
+     'k, 'l, 'm, 'n, 'o, 'p) isasat_int\<close> where
+  \<open>remove_n isasat_int = (case isasat_int of IsaSAT_int x1 x2 x3 x4 x5 x6 x7 x8 x9 x10 x11 x12 x13 x14 x15 x16 \<Rightarrow>
+      (x14, IsaSAT_int x1 x2 x3 x4 x5 x6 x7 x8 x9 x10 x11 x12 x13 n_default x15 x16))\<close>
+
+definition remove_o :: \<open>('a, 'b, 'c, 'd, 'e, 'f, 'g, 'h, 'i, 'j,
+     'k, 'l, 'm, 'n, 'o, 'p) isasat_int \<Rightarrow> 'o \<times> ('a, 'b, 'c, 'd, 'e, 'f, 'g, 'h, 'i, 'j,
+     'k, 'l, 'm, 'n, 'o, 'p) isasat_int\<close> where
+  \<open>remove_o isasat_int = (case isasat_int of IsaSAT_int x1 x2 x3 x4 x5 x6 x7 x8 x9 x10 x11 x12 x13 x14 x15 x16 \<Rightarrow>
+      (x15, IsaSAT_int x1 x2 x3 x4 x5 x6 x7 x8 x9 x10 x11 x12 x13 x14 ko_default x16))\<close>
+
+definition remove_p :: \<open>('a, 'b, 'c, 'd, 'e, 'f, 'g, 'h, 'i, 'j,
+     'k, 'l, 'm, 'n, 'o, 'p) isasat_int \<Rightarrow> 'p \<times> ('a, 'b, 'c, 'd, 'e, 'f, 'g, 'h, 'i, 'j,
+     'k, 'l, 'm, 'n, 'o, 'p) isasat_int\<close> where
+  \<open>remove_p isasat_int = (case isasat_int of IsaSAT_int x1 x2 x3 x4 x5 x6 x7 x8 x9 x10 x11 x12 x13 x14 x15 x16 \<Rightarrow>
+      (x16, IsaSAT_int x1 x2 x3 x4 x5 x6 x7 x8 x9 x10 x11 x12 x13 x14 x15 p_default))\<close>
+
+definition update_a :: \<open>'a \<Rightarrow> ('a, 'b, 'c, 'd, 'e, 'f, 'g, 'h, 'i, 'j,
+     'k, 'l, 'm, 'n, 'o, 'p) isasat_int \<Rightarrow> ('a, 'b, 'c, 'd, 'e, 'f, 'g, 'h, 'i, 'j,
+     'k, 'l, 'm, 'n, 'o, 'p) isasat_int\<close> where
+  \<open>update_a x1 isasat_int = (case isasat_int of IsaSAT_int M x2 x3 x4 x5 x6 x7 x8 x9 x10 x11 x12 x13 x14 x15 x16 \<Rightarrow>
+    let _ = M in
+    IsaSAT_int x1 x2 x3 x4 x5 x6 x7 x8 x9 x10 x11 x12 x13 x14 x15 x16)\<close>
+
+definition update_b :: \<open>'b \<Rightarrow> ('a, 'b, 'c, 'd, 'e, 'f, 'g, 'h, 'i, 'j,
+     'k, 'l, 'm, 'n, 'o, 'p) isasat_int \<Rightarrow> ('a, 'b, 'c, 'd, 'e, 'f, 'g, 'h, 'i, 'j,
+     'k, 'l, 'm, 'n, 'o, 'p) isasat_int\<close> where
+  \<open>update_b x2 isasat_int = (case isasat_int of IsaSAT_int x1 M x3 x4 x5 x6 x7 x8 x9 x10 x11 x12 x13 x14 x15 x16 \<Rightarrow>
+    let _ = M in
+    IsaSAT_int x1 x2 x3 x4 x5 x6 x7 x8 x9 x10 x11 x12 x13 x14 x15 x16)\<close>
+
+definition update_c:: \<open>'c \<Rightarrow> ('a, 'b, 'c, 'd, 'e, 'f, 'g, 'h, 'i, 'j,
+     'k, 'l, 'm, 'n, 'o, 'p) isasat_int \<Rightarrow> ('a, 'b, 'c, 'd, 'e, 'f, 'g, 'h, 'i, 'j,
+     'k, 'l, 'm, 'n, 'o, 'p) isasat_int\<close> where
+  \<open>update_c x3 isasat_int = (case isasat_int of IsaSAT_int x1 x2 M x4 x5 x6 x7 x8 x9 x10 x11 x12 x13 x14 x15 x16 \<Rightarrow>
+    let _ = M in
+    IsaSAT_int x1 x2 x3 x4 x5 x6 x7 x8 x9 x10 x11 x12 x13 x14 x15 x16)\<close>
+
+definition update_d :: \<open>'d \<Rightarrow> ('a, 'b, 'c, 'd, 'e, 'f, 'g, 'h, 'i, 'j,
+     'k, 'l, 'm, 'n, 'o, 'p) isasat_int \<Rightarrow> ('a, 'b, 'c, 'd, 'e, 'f, 'g, 'h, 'i, 'j,
+     'k, 'l, 'm, 'n, 'o, 'p) isasat_int\<close> where
+  \<open>update_d x4 isasat_int = (case isasat_int of IsaSAT_int x1 x2 x3 M x5 x6 x7 x8 x9 x10 x11 x12 x13 x14 x15 x16 \<Rightarrow>
+    let _ = M in
+    IsaSAT_int x1 x2 x3 x4 x5 x6 x7 x8 x9 x10 x11 x12 x13 x14 x15 x16)\<close>
+
+definition update_e :: \<open>'e \<Rightarrow> ('a, 'b, 'c, 'd, 'e, 'f, 'g, 'h, 'i, 'j,
+     'k, 'l, 'm, 'n, 'o, 'p) isasat_int \<Rightarrow> ('a, 'b, 'c, 'd, 'e, 'f, 'g, 'h, 'i, 'j,
+     'k, 'l, 'm, 'n, 'o, 'p) isasat_int\<close> where
+  \<open>update_e x5 isasat_int = (case isasat_int of IsaSAT_int x1 x2 x3 x4 M x6 x7 x8 x9 x10 x11 x12 x13 x14 x15 x16 \<Rightarrow>
+    let _ = M in
+    IsaSAT_int x1 x2 x3 x4 x5 x6 x7 x8 x9 x10 x11 x12 x13 x14 x15 x16)\<close>
+
+definition update_f :: \<open>'f \<Rightarrow> ('a, 'b, 'c, 'd, 'e, 'f, 'g, 'h, 'i, 'j,
+     'k, 'l, 'm, 'n, 'o, 'p) isasat_int \<Rightarrow> ('a, 'b, 'c, 'd, 'e, 'f, 'g, 'h, 'i, 'j,
+     'k, 'l, 'm, 'n, 'o, 'p) isasat_int\<close> where
+  \<open>update_f x6 isasat_int = (case isasat_int of IsaSAT_int x1 x2 x3 x4 x5 M x7 x8 x9 x10 x11 x12 x13 x14 x15 x16 \<Rightarrow>
+    let _ = M in
+    IsaSAT_int x1 x2 x3 x4 x5 x6 x7 x8 x9 x10 x11 x12 x13 x14 x15 x16)\<close>
+
+definition update_g :: \<open>'g \<Rightarrow> ('a, 'b, 'c, 'd, 'e, 'f, 'g, 'h, 'i, 'j,
+     'k, 'l, 'm, 'n, 'o, 'p) isasat_int \<Rightarrow> ('a, 'b, 'c, 'd, 'e, 'f, 'g, 'h, 'i, 'j,
+     'k, 'l, 'm, 'n, 'o, 'p) isasat_int\<close> where
+  \<open>update_g x7 isasat_int = (case isasat_int of IsaSAT_int x1 x2 x3 x4 x5 x6 M x8 x9 x10 x11 x12 x13 x14 x15 x16 \<Rightarrow>
+    let _ = M in
+    IsaSAT_int x1 x2 x3 x4 x5 x6 x7 x8 x9 x10 x11 x12 x13 x14 x15 x16)\<close>
+
+definition update_h :: \<open>'h \<Rightarrow> ('a, 'b, 'c, 'd, 'e, 'f, 'g, 'h, 'i, 'j,
+     'k, 'l, 'm, 'n, 'o, 'p) isasat_int \<Rightarrow> ('a, 'b, 'c, 'd, 'e, 'f, 'g, 'h, 'i, 'j,
+     'k, 'l, 'm, 'n, 'o, 'p) isasat_int\<close> where
+  \<open>update_h x8 isasat_int = (case isasat_int of IsaSAT_int x1 x2 x3 x4 x5 x6 x7 M x9 x10 x11 x12 x13 x14 x15 x16 \<Rightarrow>
+    let _ = M in
+    IsaSAT_int x1 x2 x3 x4 x5 x6 x7 x8 x9 x10 x11 x12 x13 x14 x15 x16)\<close>
+
+definition update_i :: \<open>'i \<Rightarrow> ('a, 'b, 'c, 'd, 'e, 'f, 'g, 'h, 'i, 'j,
+     'k, 'l, 'm, 'n, 'o, 'p) isasat_int \<Rightarrow> ('a, 'b, 'c, 'd, 'e, 'f, 'g, 'h, 'i, 'j,
+     'k, 'l, 'm, 'n, 'o, 'p) isasat_int\<close> where
+  \<open>update_i x9 isasat_int = (case isasat_int of IsaSAT_int x1 x2 x3 x4 x5 x6 x7 x8 M x10 x11 x12 x13 x14 x15 x16 \<Rightarrow>
+    let _ = M in
+    IsaSAT_int x1 x2 x3 x4 x5 x6 x7 x8 x9 x10 x11 x12 x13 x14 x15 x16)\<close>
+
+definition update_j :: \<open>'j \<Rightarrow> ('a, 'b, 'c, 'd, 'e, 'f, 'g, 'h, 'i, 'j,
+     'k, 'l, 'm, 'n, 'o, 'p) isasat_int \<Rightarrow> ('a, 'b, 'c, 'd, 'e, 'f, 'g, 'h, 'i, 'j,
+     'k, 'l, 'm, 'n, 'o, 'p) isasat_int\<close> where
+  \<open>update_j x10 isasat_int = (case isasat_int of IsaSAT_int x1 x2 x3 x4 x5 x6 x7 x8 x9 M x11 x12 x13 x14 x15 x16 \<Rightarrow>
+    let _ = M in
+    IsaSAT_int x1 x2 x3 x4 x5 x6 x7 x8 x9 x10 x11 x12 x13 x14 x15 x16)\<close>
+
+definition update_k :: \<open>'k \<Rightarrow> ('a, 'b, 'c, 'd, 'e, 'f, 'g, 'h, 'i, 'j,
+     'k, 'l, 'm, 'n, 'o, 'p) isasat_int \<Rightarrow> ('a, 'b, 'c, 'd, 'e, 'f, 'g, 'h, 'i, 'j,
+     'k, 'l, 'm, 'n, 'o, 'p) isasat_int\<close> where
+  \<open>update_k x11 isasat_int = (case isasat_int of IsaSAT_int x1 x2 x3 x4 x5 x6 x7 x8 x9 x10 M x12 x13 x14 x15 x16 \<Rightarrow>
+    let _ = M in
+    IsaSAT_int x1 x2 x3 x4 x5 x6 x7 x8 x9 x10 x11 x12 x13 x14 x15 x16)\<close>
+
+definition update_l :: \<open>'l \<Rightarrow> ('a, 'b, 'c, 'd, 'e, 'f, 'g, 'h, 'i, 'j,
+     'k, 'l, 'm, 'n, 'o, 'p) isasat_int \<Rightarrow> ('a, 'b, 'c, 'd, 'e, 'f, 'g, 'h, 'i, 'j,
+     'k, 'l, 'm, 'n, 'o, 'p) isasat_int\<close> where
+  \<open>update_l x12 isasat_int = (case isasat_int of IsaSAT_int x1 x2 x3 x4 x5 x6 x7 x8 x9 x10 x11 M x13 x14 x15 x16 \<Rightarrow>
+    let _ = M in
+    IsaSAT_int x1 x2 x3 x4 x5 x6 x7 x8 x9 x10 x11 x12 x13 x14 x15 x16)\<close>
+
+definition update_m :: \<open>'m \<Rightarrow> ('a, 'b, 'c, 'd, 'e, 'f, 'g, 'h, 'i, 'j,
+     'k, 'l, 'm, 'n, 'o, 'p) isasat_int \<Rightarrow> ('a, 'b, 'c, 'd, 'e, 'f, 'g, 'h, 'i, 'j,
+     'k, 'l, 'm, 'n, 'o, 'p) isasat_int\<close> where
+  \<open>update_m x13 isasat_int = (case isasat_int of IsaSAT_int x1 x2 x3 x4 x5 x6 x7 x8 x9 x10 x11 x12 M x14 x15 x16 \<Rightarrow>
+    let _ = M in
+    IsaSAT_int x1 x2 x3 x4 x5 x6 x7 x8 x9 x10 x11 x12 x13 x14 x15 x16)\<close>
+
+definition update_n :: \<open>'n \<Rightarrow> ('a, 'b, 'c, 'd, 'e, 'f, 'g, 'h, 'i, 'j,
+     'k, 'l, 'm, 'n, 'o, 'p) isasat_int \<Rightarrow> ('a, 'b, 'c, 'd, 'e, 'f, 'g, 'h, 'i, 'j,
+     'k, 'l, 'm, 'n, 'o, 'p) isasat_int\<close> where
+  \<open>update_n x14 isasat_int = (case isasat_int of IsaSAT_int x1 x2 x3 x4 x5 x6 x7 x8 x9 x10 x11 x12 x13 M x15 x16 \<Rightarrow>
+    let _ = M in
+    IsaSAT_int x1 x2 x3 x4 x5 x6 x7 x8 x9 x10 x11 x12 x13 x14 x15 x16)\<close>
+
+definition update_o :: \<open>'o \<Rightarrow> ('a, 'b, 'c, 'd, 'e, 'f, 'g, 'h, 'i, 'j,
+     'k, 'l, 'm, 'n, 'o, 'p) isasat_int \<Rightarrow> ('a, 'b, 'c, 'd, 'e, 'f, 'g, 'h, 'i, 'j,
+     'k, 'l, 'm, 'n, 'o, 'p) isasat_int\<close> where
+  \<open>update_o x15 isasat_int = (case isasat_int of IsaSAT_int x1 x2 x3 x4 x5 x6 x7 x8 x9 x10 x11 x12 x13 x14 M x16 \<Rightarrow>
+    let _ = M in
+    IsaSAT_int x1 x2 x3 x4 x5 x6 x7 x8 x9 x10 x11 x12 x13 x14 x15 x16)\<close>
+
+
+definition update_p :: \<open>'p \<Rightarrow> ('a, 'b, 'c, 'd, 'e, 'f, 'g, 'h, 'i, 'j,
+     'k, 'l, 'm, 'n, 'o, 'p) isasat_int \<Rightarrow> ('a, 'b, 'c, 'd, 'e, 'f, 'g, 'h, 'i, 'j,
+     'k, 'l, 'm, 'n, 'o, 'p) isasat_int\<close> where
+  \<open>update_p x16 isasat_int = (case isasat_int of IsaSAT_int x1 x2 x3 x4 x5 x6 x7 x8 x9 x10 x11 x12 x13 x14 x15 M \<Rightarrow>
+    let _ = M in
+    IsaSAT_int x1 x2 x3 x4 x5 x6 x7 x8 x9 x10 x11 x12 x13 x14 x15 x16)\<close>
+
+
+end
+
+lemma isasat_int_assn_conv[simp]:
+  "isasat_int_assn P1 P2 P3 P4 P5 P6 P7 P8 P9 P10 P11 P12 P13 P14 P15 P16 (IsaSAT_int a1 a2 a3 a4 a5 a6 a7 a8 a9 a10 a11 a12 a13 a14 a15 a16)
+  (IsaSAT_int a1' a2' a3' a4' a5' a6' a7' a8' a9' a10' a11' a12' a13' a14' a15' a16') =
+  (P1 a1 a1' \<and>*
+  P2 a2 a2' \<and>*
+  P3 a3 a3' \<and>*
+  P4 a4 a4' \<and>*
+  P5 a5 a5' \<and>*
+  P6 a6 a6' \<and>*
+  P7 a7 a7' \<and>*
+  P8 a8 a8' \<and>* P9 a9 a9' \<and>* P10 a10 a10' \<and>* P11 a11 a11' \<and>* P12 a12 a12' \<and>* P13 a13 a13' \<and>* P14 a14 a14' \<and>* P15 a15 a15' \<and>* P16 a16 a16')"
+  unfolding isasat_int_assn.simps by auto
+lemma isasat_int_assn_ctxt:
+  \<open>isasat_int_assn P1 P2 P3 P4 P5 P6 P7 P8 P9 P10 P11 P12 P13 P14 P15 P16 (IsaSAT_int a1 a2 a3 a4 a5 a6 a7 a8 a9 a10 a11 a12 a13 a14 a15 a16)
+  (IsaSAT_int a1' a2' a3' a4' a5' a6' a7' a8' a9' a10' a11' a12' a13' a14' a15' a16') = z \<Longrightarrow>
+  hn_ctxt (isasat_int_assn P1 P2 P3 P4 P5 P6 P7 P8 P9 P10 P11 P12 P13 P14 P15 P16) (IsaSAT_int a1 a2 a3 a4 a5 a6 a7 a8 a9 a10 a11 a12 a13 a14 a15 a16)
+  (IsaSAT_int a1' a2' a3' a4' a5' a6' a7' a8' a9' a10' a11' a12' a13' a14' a15' a16')= z\<close>
+  by (simp add: hn_ctxt_def)
+
+lemma hn_case_isasat_int'[sepref_comb_rules]:
+  assumes FR: \<open>\<Gamma> \<turnstile> hn_ctxt (isasat_int_assn P1 P2 P3 P4 P5 P6 P7 P8 P9 P10 P11 P12 P13 P14 P15 P16) p' p ** \<Gamma>1\<close>
+  assumes Pair: "\<And>a1 a2 a3 a4 a5 a6 a7 a8 a9 a10 a11 a12 a13 a14 a15 a16 a1' a2' a3' a4' a5' a6' a7' a8' a9' a10' a11' a12' a13' a14' a15' a16'.
+        \<lbrakk>p'=IsaSAT_int a1' a2' a3' a4' a5' a6' a7' a8' a9' a10' a11' a12' a13' a14' a15' a16'\<rbrakk>
+    \<Longrightarrow> hn_refine (hn_ctxt P1 a1' a1 \<and>* hn_ctxt P2 a2' a2 \<and>* hn_ctxt P3 a3' a3 \<and>* hn_ctxt P4 a4' a4 \<and>*
+       hn_ctxt P5 a5' a5 \<and>* hn_ctxt P6 a6' a6 \<and>* hn_ctxt P7 a7' a7 \<and>* hn_ctxt P8 a8' a8 \<and>*
+       hn_ctxt P9 a9' a9 \<and>* hn_ctxt P10 a10' a10 \<and>* hn_ctxt P11 a11' a11 \<and>* hn_ctxt P12 a12' a12 \<and>*
+       hn_ctxt P13 a13' a13 \<and>* hn_ctxt P14 a14' a14 \<and>* hn_ctxt P15 a15' a15 \<and>* hn_ctxt P16 a16' a16 \<and>* \<Gamma>1)
+          (f a1 a2 a3 a4 a5 a6 a7 a8 a9 a10 a11 a12 a13 a14 a15 a16)
+          (\<Gamma>2 a1 a2 a3 a4 a5 a6 a7 a8 a9 a10 a11 a12 a13 a14 a15 a16 a1' a2' a3' a4' a5' a6' a7' a8' a9' a10' a11' a12' a13' a14' a15' a16') R
+          (CP a1 a2  a3 a4 a5 a6 a7 a8 a9 a10 a11 a12 a13 a14 a15 a16)
+         (f' a1' a2' a3' a4' a5' a6' a7' a8' a9' a10' a11' a12' a13' a14' a15' a16')"
+  assumes FR2: \<open>\<And>a1 a2 a3 a4 a5 a6 a7 a8 a9 a10 a11 a12 a13 a14 a15 a16 a1' a2' a3' a4' a5' a6' a7' a8' a9' a10' a11' a12' a13' a14' a15' a16'.
+       \<Gamma>2 a1 a2 a3 a4 a5 a6 a7 a8 a9 a10 a11 a12 a13 a14 a15 a16 a1' a2' a3' a4' a5' a6' a7' a8' a9' a10' a11' a12' a13' a14' a15' a16' \<turnstile>
+       hn_ctxt P1' a1' a1 ** hn_ctxt P2' a2' a2 ** hn_ctxt P3' a3' a3 ** hn_ctxt P4' a4' a4 **
+       hn_ctxt P5' a5' a5 ** hn_ctxt P6' a6' a6 ** hn_ctxt P7' a7' a7 ** hn_ctxt P8' a8' a8 **
+       hn_ctxt P9' a9' a9 ** hn_ctxt P10' a10' a10 ** hn_ctxt P11' a11' a11 ** hn_ctxt P12' a12' a12 **
+       hn_ctxt P13' a13' a13 ** hn_ctxt P14' a14' a14 ** hn_ctxt P15' a15' a15 ** hn_ctxt P16' a16' a16 ** \<Gamma>1'\<close>
+  shows \<open>hn_refine \<Gamma> (case_isasat_int f p) (hn_ctxt (isasat_int_assn P1' P2' P3' P4' P5' P6' P7' P8' P9' P10' P11' P12' P13' P14' P15' P16') p' p ** \<Gamma>1')
+    R (case_isasat_int CP p) (case_isasat_int$(\<lambda>\<^sub>2a1 a2 a3 a4 a5 a6 a7 a8 a9 a10 a11 a12 a13 a14 a15 a16. f' a1 a2 a3 a4 a5 a6 a7 a8 a9 a10 a11 a12 a13 a14 a15 a16)$p')\<close> (is \<open>?G \<Gamma>\<close>)
+  unfolding autoref_tag_defs PROTECT2_def
+  apply1 (rule hn_refine_cons_pre[OF FR])
+    apply1 (cases p; cases p'; simp add: isasat_int_assn_conv[THEN isasat_int_assn_ctxt])
+  unfolding CP_SPLIT_def prod.simps
+  apply (rule hn_refine_cons[OF _ Pair _ entails_refl])
+  applyS (simp add: hn_ctxt_def)
+  applyS simp using FR2
+  by (simp add: hn_ctxt_def)
+
+
+lemma case_isasat_int_arity[sepref_monadify_arity]:
+  \<open>case_isasat_int \<equiv> \<lambda>\<^sub>2fp p. SP case_isasat_int$(\<lambda>\<^sub>2a b. fp$a$b)$p\<close>
+  by (simp_all only: SP_def APP_def PROTECT2_def RCALL_def)
+
+lemma case_isasat_int_comb[sepref_monadify_comb]:
+  \<open>\<And>fp p. case_isasat_int$fp$p \<equiv> Refine_Basic.bind$(EVAL$p)$(\<lambda>\<^sub>2p. (SP case_isasat_int$fp$p))\<close>
+  by (simp_all)
+
+lemma case_isasat_int_plain_comb[sepref_monadify_comb]:
+  "EVAL$(case_isasat_int$(\<lambda>\<^sub>2a1 a2 a3 a4 a5 a6 a7 a8 a9 a10 a11 a12 a13 a14 a15 a16. fp a1 a2 a3 a4 a5 a6 a7 a8 a9 a10 a11 a12 a13 a14 a15 a16)$p) \<equiv>
+    Refine_Basic.bind$(EVAL$p)$(\<lambda>\<^sub>2p. case_isasat_int$(\<lambda>\<^sub>2a1 a2 a3 a4 a5 a6 a7 a8 a9 a10 a11 a12 a13 a14 a15 a16. EVAL$(fp a1 a2 a3 a4 a5 a6 a7 a8 a9 a10 a11 a12 a13 a14 a15 a16))$p)"
+  apply (rule eq_reflection, simp split: list.split prod.split option.split isasat_int.split)+
+  done
+
+lemma ho_isasat_int_move[sepref_preproc]: \<open>case_isasat_int (\<lambda>a1 a2 a3 a4 a5 a6 a7 a8 a9 a10 a11 a12 a13 a14 a15 a16 x. f x a1 a2 a3 a4 a5 a6 a7 a8 a9 a10 a11 a12 a13 a14 a15 a16) =
+  (\<lambda>p x. case_isasat_int (f x) p)\<close>
+  by (auto split: isasat_int.splits)
+
+locale isasat_state =
+  isasat_state_ops a_assn b_assn c_assn d_assn e_assn
+  f_assn g_assn h_assn i_assn j_assn
+  k_assn l_assn m_assn n_assn o_assn p_assn
+  a_default a
+  b_default b
+  c_default c
+  d_default d
+  e_default e
+  f_default f
+  g_default g
+  h_default h
+  i_default i
+  j_default j
+  k_default k
+  l_default l
+  m_default m
+  n_default n
+  ko_default ko
+  p_default p
+  for
+    a_assn :: \<open>'a \<Rightarrow> 'xa \<Rightarrow> assn\<close> and
+    b_assn :: \<open>'b \<Rightarrow> 'xb \<Rightarrow> assn\<close> and
+    c_assn :: \<open>'c \<Rightarrow> 'xc \<Rightarrow> assn\<close> and
+    d_assn :: \<open>'d \<Rightarrow> 'xd \<Rightarrow> assn\<close> and
+    e_assn :: \<open>'e \<Rightarrow> 'xe \<Rightarrow> assn\<close> and
+    f_assn :: \<open>'f \<Rightarrow> 'xf \<Rightarrow> assn\<close> and
+    g_assn :: \<open>'g \<Rightarrow> 'xg \<Rightarrow> assn\<close> and
+    h_assn :: \<open>'h \<Rightarrow> 'xh \<Rightarrow> assn\<close> and
+    i_assn :: \<open>'i \<Rightarrow> 'xi \<Rightarrow> assn\<close> and
+    j_assn :: \<open>'j \<Rightarrow> 'xj \<Rightarrow> assn\<close> and
+    k_assn :: \<open>'k \<Rightarrow> 'xk \<Rightarrow> assn\<close> and
+    l_assn :: \<open>'l \<Rightarrow> 'xl \<Rightarrow> assn\<close> and
+    m_assn :: \<open>'m \<Rightarrow> 'xm \<Rightarrow> assn\<close> and
+    n_assn :: \<open>'n \<Rightarrow> 'xn \<Rightarrow> assn\<close> and
+    o_assn :: \<open>'o \<Rightarrow> 'xo \<Rightarrow> assn\<close> and
+    p_assn :: \<open>'p \<Rightarrow> 'xp \<Rightarrow> assn\<close> and
+    a_default :: 'a and
+    a :: \<open>'xa llM\<close> and
+    b_default :: 'b and
+    b :: \<open>'xb llM\<close> and
+    c_default :: 'c and
+    c :: \<open>'xc llM\<close> and
+    d_default :: 'd and
+    d :: \<open>'xd llM\<close> and
+    e_default :: 'e and
+    e :: \<open>'xe llM\<close> and
+    f_default :: 'f and
+    f :: \<open>'xf llM\<close> and
+    g_default :: 'g and
+    g :: \<open>'xg llM\<close> and
+    h_default :: 'h and
+    h :: \<open>'xh llM\<close> and
+    i_default :: 'i and
+    i :: \<open>'xi llM\<close> and
+    j_default :: 'j and
+    j :: \<open>'xj llM\<close> and
+    k_default :: 'k and
+    k :: \<open>'xk llM\<close> and
+    l_default :: 'l and
+    l :: \<open>'xl llM\<close> and
+    m_default :: 'm and
+    m :: \<open>'xm llM\<close> and
+    n_default :: 'n and
+    n :: \<open>'xn llM\<close> and
+    ko_default :: 'o and
+    ko :: \<open>'xo llM\<close> and
+    p_default :: 'p and
+    p :: \<open>'xp llM\<close> and
+    a_free :: \<open>'xa \<Rightarrow> unit llM\<close> and
+    b_free :: \<open>'xb \<Rightarrow> unit llM\<close> and
+    c_free :: \<open>'xc \<Rightarrow> unit llM\<close> and
+    d_free :: \<open>'xd \<Rightarrow> unit llM\<close> and
+    e_free :: \<open>'xe \<Rightarrow> unit llM\<close> and
+    f_free :: \<open>'xf \<Rightarrow> unit llM\<close> and
+    g_free :: \<open>'xg \<Rightarrow> unit llM\<close> and
+    h_free :: \<open>'xh \<Rightarrow> unit llM\<close> and
+    i_free :: \<open>'xi \<Rightarrow> unit llM\<close> and
+    j_free :: \<open>'xj \<Rightarrow> unit llM\<close> and
+    k_free :: \<open>'xk \<Rightarrow> unit llM\<close> and
+    l_free :: \<open>'xl \<Rightarrow> unit llM\<close> and
+    m_free :: \<open>'xm \<Rightarrow> unit llM\<close> and
+    n_free :: \<open>'xn \<Rightarrow> unit llM\<close> and
+    o_free :: \<open>'xo \<Rightarrow> unit llM\<close> and
+    p_free :: \<open>'xp \<Rightarrow> unit llM\<close> +
+  assumes
+    a: \<open>(uncurry0 a, uncurry0  (RETURN a_default)) \<in> unit_assn\<^sup>k \<rightarrow>\<^sub>a a_assn\<close> and
+    b: \<open>(uncurry0 b, uncurry0  (RETURN b_default)) \<in> unit_assn\<^sup>k \<rightarrow>\<^sub>a b_assn\<close> and
+    c: \<open>(uncurry0 c, uncurry0  (RETURN c_default)) \<in> unit_assn\<^sup>k \<rightarrow>\<^sub>a c_assn\<close> and
+    d: \<open>(uncurry0 d, uncurry0  (RETURN d_default)) \<in> unit_assn\<^sup>k \<rightarrow>\<^sub>a d_assn\<close> and
+    e: \<open>(uncurry0 e, uncurry0  (RETURN e_default)) \<in> unit_assn\<^sup>k \<rightarrow>\<^sub>a e_assn\<close> and
+    f: \<open>(uncurry0 f, uncurry0  (RETURN f_default)) \<in> unit_assn\<^sup>k \<rightarrow>\<^sub>a f_assn\<close> and
+    g: \<open>(uncurry0 g, uncurry0  (RETURN g_default)) \<in> unit_assn\<^sup>k \<rightarrow>\<^sub>a g_assn\<close> and
+    h: \<open>(uncurry0 h, uncurry0  (RETURN h_default)) \<in> unit_assn\<^sup>k \<rightarrow>\<^sub>a h_assn\<close> and
+    i: \<open>(uncurry0 i, uncurry0  (RETURN i_default)) \<in> unit_assn\<^sup>k \<rightarrow>\<^sub>a i_assn\<close> and
+    j: \<open>(uncurry0 j, uncurry0  (RETURN j_default)) \<in> unit_assn\<^sup>k \<rightarrow>\<^sub>a j_assn\<close> and
+    k: \<open>(uncurry0 k, uncurry0  (RETURN k_default)) \<in> unit_assn\<^sup>k \<rightarrow>\<^sub>a k_assn\<close> and
+    l: \<open>(uncurry0 l, uncurry0  (RETURN l_default)) \<in> unit_assn\<^sup>k \<rightarrow>\<^sub>a l_assn\<close> and
+    m: \<open>(uncurry0 m, uncurry0  (RETURN m_default)) \<in> unit_assn\<^sup>k \<rightarrow>\<^sub>a m_assn\<close> and
+    n: \<open>(uncurry0 n, uncurry0  (RETURN n_default)) \<in> unit_assn\<^sup>k \<rightarrow>\<^sub>a n_assn\<close> and
+    o: \<open>(uncurry0 ko, uncurry0  (RETURN ko_default)) \<in> unit_assn\<^sup>k \<rightarrow>\<^sub>a o_assn\<close>and
+    p: \<open>(uncurry0 p, uncurry0 (RETURN p_default)) \<in> unit_assn\<^sup>k \<rightarrow>\<^sub>a p_assn\<close> and
+    a_free: \<open>MK_FREE a_assn a_free\<close> and
+    b_free: \<open>MK_FREE b_assn b_free\<close>and
+    c_free: \<open>MK_FREE c_assn c_free\<close>and
+    d_free: \<open>MK_FREE d_assn d_free\<close>and
+    e_free: \<open>MK_FREE e_assn e_free\<close>and
+    f_free: \<open>MK_FREE f_assn f_free\<close>and
+    g_free: \<open>MK_FREE g_assn g_free\<close>and
+    h_free: \<open>MK_FREE h_assn h_free\<close>and
+    i_free: \<open>MK_FREE i_assn i_free\<close>and
+    j_free: \<open>MK_FREE j_assn j_free\<close>and
+    k_free: \<open>MK_FREE k_assn k_free\<close>and
+    l_free: \<open>MK_FREE l_assn l_free\<close>and
+    m_free: \<open>MK_FREE m_assn m_free\<close>and
+    n_free: \<open>MK_FREE n_assn n_free\<close>and
+    o_free: \<open>MK_FREE o_assn o_free\<close>and
+    p_free: \<open>MK_FREE p_assn p_free\<close>
+  notes [[sepref_register_adhoc a_default b_default c_default d_default e_default f_default g_default h_default
+  i_default j_default k_default l_default m_default n_default ko_default p_default]]
+begin
+
+lemmas [sepref_comb_rules] = hn_case_isasat_int'[of _ a_assn b_assn c_assn d_assn e_assn f_assn
+  g_assn h_assn i_assn j_assn k_assn l_assn m_assn n_assn o_assn p_assn,
+  unfolded isasat_assn_def[symmetric]]
+
+lemma ex_isasat_int_iff: "(\<exists>b :: (_,_,_,_,_,_,_,_,_,_,_,_,_,_,_,_)isasat_int. P b) \<longleftrightarrow>
+  (\<exists>a b  c d e f g h i j k l m n ko p. P (IsaSAT_int a b  c d e f g h i j k l m n ko p))"
+  apply auto
+    apply (case_tac b)
+  by force
+
+lemmas [sepref_frame_free_rules] = a_free b_free c_free d_free e_free f_free g_free h_free i_free
+  j_free k_free l_free m_free n_free o_free p_free
+sepref_register
+  \<open>IsaSAT_int\<close>
+lemma [sepref_fr_rules]: \<open>(uncurry15 (Mreturn o\<^sub>1\<^sub>6 IsaSAT_int), uncurry15 (RETURN o\<^sub>1\<^sub>6 IsaSAT_int))
+  \<in> a_assn\<^sup>d *\<^sub>a b_assn\<^sup>d *\<^sub>a c_assn\<^sup>d *\<^sub>a d_assn\<^sup>d *\<^sub>a
+  e_assn\<^sup>d *\<^sub>a f_assn\<^sup>d *\<^sub>a g_assn\<^sup>d *\<^sub>a h_assn\<^sup>d *\<^sub>a
+  i_assn\<^sup>d *\<^sub>a j_assn\<^sup>d *\<^sub>a k_assn\<^sup>d *\<^sub>a l_assn\<^sup>d *\<^sub>a
+  m_assn\<^sup>d *\<^sub>a n_assn\<^sup>d *\<^sub>a o_assn\<^sup>d *\<^sub>a p_assn\<^sup>d
+  \<rightarrow>\<^sub>a isasat_assn\<close>
+  unfolding isasat_assn_def
+  apply sepref_to_hoare
+  apply vcg
+  unfolding ex_isasat_int_iff
+  apply vcg'
+  done
+
+lemma [sepref_frame_match_rules]:
+  \<open> hn_ctxt
+     (isasat_int_assn (invalid_assn a_assn) (invalid_assn b_assn) (invalid_assn c_assn) (invalid_assn d_assn) (invalid_assn e_assn)
+    (invalid_assn f_assn) (invalid_assn g_assn) (invalid_assn h_assn) (invalid_assn i_assn) (invalid_assn j_assn) (invalid_assn k_assn)
+   (invalid_assn l_assn) (invalid_assn m_assn) (invalid_assn n_assn) (invalid_assn o_assn) (invalid_assn p_assn)) ax bx \<turnstile> hn_val UNIV ax bx\<close>
+    unfolding hn_ctxt_def invalid_assn_def isasat_assn_def entails_def
+    apply (auto split: prod.split isasat_int.splits elim: is_pureE
+      simp: sep_algebra_simps pure_part_pure_conj_eq)
+    apply (auto simp: pure_part_def)
+      apply (auto simp: pure_def pure_true_conv)
+    done
+
+lemma RETURN_case_isasat_int_inverse: \<open>RETURN
+      (let _ = M
+         in ff) =
+      (do {_ \<leftarrow> mop_free M;
+         RETURN (ff)})\<close>
+    by (auto intro!: ext simp: mop_free_def split: isasat_int.splits)
+
+sepref_def update_a_code
+  is \<open>uncurry (RETURN oo update_a)\<close>
+  :: \<open>a_assn\<^sup>d *\<^sub>a isasat_assn\<^sup>d \<rightarrow>\<^sub>a isasat_assn\<close>
+  supply [[goals_limit=5]]
+  unfolding update_a_def isasat_int.case_distrib comp_def RETURN_case_isasat_int_inverse
+  by sepref
+
+sepref_def update_b_code
+  is \<open>uncurry (RETURN oo update_b)\<close>
+  :: \<open>b_assn\<^sup>d *\<^sub>a isasat_assn\<^sup>d \<rightarrow>\<^sub>a isasat_assn\<close>
+  supply [[goals_limit=1]]
+  unfolding update_b_def isasat_int.case_distrib comp_def RETURN_case_isasat_int_inverse
+  by sepref
+
+sepref_def update_c_code
+  is \<open>uncurry (RETURN oo update_c)\<close>
+  :: \<open>c_assn\<^sup>d *\<^sub>a isasat_assn\<^sup>d \<rightarrow>\<^sub>a isasat_assn\<close>
+  supply [[goals_limit=1]]
+  unfolding update_c_def isasat_int.case_distrib comp_def RETURN_case_isasat_int_inverse
+  by sepref
+
+sepref_def update_d_code
+  is \<open>uncurry (RETURN oo update_d)\<close>
+  :: \<open>d_assn\<^sup>d *\<^sub>a isasat_assn\<^sup>d \<rightarrow>\<^sub>a isasat_assn\<close>
+  supply [[goals_limit=1]]
+  unfolding update_d_def isasat_int.case_distrib comp_def RETURN_case_isasat_int_inverse
+  by sepref
+
+sepref_def update_e_code
+  is \<open>uncurry (RETURN oo update_e)\<close>
+  :: \<open>e_assn\<^sup>d *\<^sub>a isasat_assn\<^sup>d \<rightarrow>\<^sub>a isasat_assn\<close>
+  supply [[goals_limit=1]]
+  unfolding update_e_def isasat_int.case_distrib comp_def RETURN_case_isasat_int_inverse
+  by sepref
+
+sepref_def update_f_code
+  is \<open>uncurry (RETURN oo update_f)\<close>
+  :: \<open>f_assn\<^sup>d *\<^sub>a isasat_assn\<^sup>d \<rightarrow>\<^sub>a isasat_assn\<close>
+  supply [[goals_limit=1]]
+  unfolding update_f_def isasat_int.case_distrib comp_def RETURN_case_isasat_int_inverse
+  by sepref
+
+sepref_def update_g_code
+  is \<open>uncurry (RETURN oo update_g)\<close>
+  :: \<open>g_assn\<^sup>d *\<^sub>a isasat_assn\<^sup>d \<rightarrow>\<^sub>a isasat_assn\<close>
+  supply [[goals_limit=1]]
+  unfolding update_g_def isasat_int.case_distrib comp_def RETURN_case_isasat_int_inverse
+  by sepref
+
+sepref_def update_h_code
+  is \<open>uncurry (RETURN oo update_h)\<close>
+  :: \<open>h_assn\<^sup>d *\<^sub>a isasat_assn\<^sup>d \<rightarrow>\<^sub>a isasat_assn\<close>
+  supply [[goals_limit=1]]
+  unfolding update_h_def isasat_int.case_distrib comp_def RETURN_case_isasat_int_inverse
+  by sepref
+
+sepref_def update_i_code
+  is \<open>uncurry (RETURN oo update_i)\<close>
+  :: \<open>i_assn\<^sup>d *\<^sub>a isasat_assn\<^sup>d \<rightarrow>\<^sub>a isasat_assn\<close>
+  supply [[goals_limit=1]]
+  unfolding update_i_def isasat_int.case_distrib comp_def RETURN_case_isasat_int_inverse
+  by sepref
+
+sepref_def update_j_code
+  is \<open>uncurry (RETURN oo update_j)\<close>
+  :: \<open>j_assn\<^sup>d *\<^sub>a isasat_assn\<^sup>d \<rightarrow>\<^sub>a isasat_assn\<close>
+  supply [[goals_limit=1]]
+  unfolding update_j_def isasat_int.case_distrib comp_def RETURN_case_isasat_int_inverse
+  by sepref
+
+sepref_def update_k_code
+  is \<open>uncurry (RETURN oo update_k)\<close>
+  :: \<open>k_assn\<^sup>d *\<^sub>a isasat_assn\<^sup>d \<rightarrow>\<^sub>a isasat_assn\<close>
+  supply [[goals_limit=1]]
+  unfolding update_k_def isasat_int.case_distrib comp_def RETURN_case_isasat_int_inverse
+  by sepref
+
+sepref_def update_l_code
+  is \<open>uncurry (RETURN oo update_l)\<close>
+  :: \<open>l_assn\<^sup>d *\<^sub>a isasat_assn\<^sup>d \<rightarrow>\<^sub>a isasat_assn\<close>
+  supply [[goals_limit=1]]
+  unfolding update_l_def isasat_int.case_distrib comp_def RETURN_case_isasat_int_inverse
+  by sepref
+
+sepref_def update_m_code
+  is \<open>uncurry (RETURN oo update_m)\<close>
+  :: \<open>m_assn\<^sup>d *\<^sub>a isasat_assn\<^sup>d \<rightarrow>\<^sub>a isasat_assn\<close>
+  supply [[goals_limit=1]]
+  unfolding update_m_def isasat_int.case_distrib comp_def RETURN_case_isasat_int_inverse
+  by sepref
+
+sepref_def update_n_code
+  is \<open>uncurry (RETURN oo update_n)\<close>
+  :: \<open>n_assn\<^sup>d *\<^sub>a isasat_assn\<^sup>d \<rightarrow>\<^sub>a isasat_assn\<close>
+  supply [[goals_limit=1]]
+  unfolding update_n_def isasat_int.case_distrib comp_def RETURN_case_isasat_int_inverse
+  by sepref
+
+sepref_def update_o_code
+  is \<open>uncurry (RETURN oo update_o)\<close>
+  :: \<open>o_assn\<^sup>d *\<^sub>a isasat_assn\<^sup>d \<rightarrow>\<^sub>a isasat_assn\<close>
+  supply [[goals_limit=1]]
+  unfolding update_o_def isasat_int.case_distrib comp_def RETURN_case_isasat_int_inverse
+  by sepref
+
+sepref_def update_p_code
+  is \<open>uncurry (RETURN oo update_p)\<close>
+  :: \<open>p_assn\<^sup>d *\<^sub>a isasat_assn\<^sup>d \<rightarrow>\<^sub>a isasat_assn\<close>
+  supply [[goals_limit=1]]
+  unfolding update_p_def isasat_int.case_distrib comp_def RETURN_case_isasat_int_inverse
+  by sepref
+
+method stuff_pre =
+    sepref_to_hoare;
+    case_tac x;
+    vcg;
+    unfold wpa_return;
+    subst (asm)(2) sep_algebra_class.sep_conj_empty'[symmetric];
+    rule apply_htriple_rule
+
+method stuff_post1 =
+    rule POSTCONDI;
+    rule STATE_monoI
+
+method stuff_post2 =
+    unfold ex_isasat_int_iff entails_def;
+    auto simp: Exists_eq_simp ex_isasat_int_iff  entails_def entails_eq_iff pure_true_conv sep_conj_left_commute;
+    smt (z3) entails_def entails_eq_iff pure_true_conv sep_conj_aci(4) sep_conj_aci(5) sep_conj_left_commute
+
+lemma RETURN_case_isasat_int_invers: \<open>(RETURN \<circ>\<circ> case_isasat_int)
+   (\<lambda>x1 x2 x3 x4 x5 x6 x7 x8 x9 x10 x11 x12 x13 x14 x15 x16.
+  ff x1 x2 x3 x4 x5 x6 x7 x8 x9 x10 x11 x12 x13 x14 x15 x16) =
+  case_isasat_int
+   (\<lambda>x1 x2 x3 x4 x5 x6 x7 x8 x9 x10 x11 x12 x13 x14 x15 x16.
+  RETURN (ff x1 x2 x3 x4 x5 x6 x7 x8 x9 x10 x11 x12 x13 x14 x15 x16))\<close>
+  by (auto intro!: ext split: isasat_int.splits)
+
+lemmas [sepref_fr_rules] = a b c d e f g h i j k l m n  o p
+
+sepref_definition remove_a_code
+  is \<open>RETURN o remove_a\<close>
+  :: \<open> isasat_assn\<^sup>d \<rightarrow>\<^sub>a a_assn \<times>\<^sub>a isasat_assn\<close>
+  unfolding remove_a_def RETURN_case_isasat_int_invers
+  by sepref
+
+sepref_definition remove_b_code
+  is \<open>RETURN o remove_b\<close>
+  :: \<open> isasat_assn\<^sup>d \<rightarrow>\<^sub>a b_assn \<times>\<^sub>a isasat_assn\<close>
+  unfolding remove_b_def RETURN_case_isasat_int_invers
+  by sepref
+
+sepref_definition remove_c_code
+  is \<open>RETURN o remove_c\<close>
+  :: \<open> isasat_assn\<^sup>d \<rightarrow>\<^sub>a c_assn \<times>\<^sub>a isasat_assn\<close>
+  unfolding remove_c_def RETURN_case_isasat_int_invers
+  by sepref
+
+sepref_definition remove_d_code
+  is \<open>RETURN o remove_d\<close>
+  :: \<open> isasat_assn\<^sup>d \<rightarrow>\<^sub>a d_assn \<times>\<^sub>a isasat_assn\<close>
+  unfolding remove_d_def RETURN_case_isasat_int_invers
+  by sepref
+
+sepref_definition remove_e_code
+  is \<open>RETURN o remove_e\<close>
+  :: \<open> isasat_assn\<^sup>d \<rightarrow>\<^sub>a e_assn \<times>\<^sub>a isasat_assn\<close>
+  unfolding remove_e_def RETURN_case_isasat_int_invers
+  by sepref
+
+sepref_definition remove_f_code
+  is \<open>RETURN o remove_f\<close>
+  :: \<open> isasat_assn\<^sup>d \<rightarrow>\<^sub>a f_assn \<times>\<^sub>a isasat_assn\<close>
+  unfolding remove_f_def RETURN_case_isasat_int_invers
+  by sepref
+
+sepref_definition remove_g_code
+  is \<open>RETURN o remove_g\<close>
+  :: \<open> isasat_assn\<^sup>d \<rightarrow>\<^sub>a g_assn \<times>\<^sub>a isasat_assn\<close>
+  unfolding remove_g_def RETURN_case_isasat_int_invers
+  by sepref
+
+sepref_definition remove_h_code
+  is \<open>RETURN o remove_h\<close>
+  :: \<open> isasat_assn\<^sup>d \<rightarrow>\<^sub>a h_assn \<times>\<^sub>a isasat_assn\<close>
+  unfolding remove_h_def RETURN_case_isasat_int_invers
+  by sepref
+
+sepref_definition remove_i_code
+  is \<open>RETURN o remove_i\<close>
+  :: \<open> isasat_assn\<^sup>d \<rightarrow>\<^sub>a i_assn \<times>\<^sub>a isasat_assn\<close>
+  unfolding remove_i_def RETURN_case_isasat_int_invers
+  by sepref
+
+sepref_definition remove_j_code
+  is \<open>RETURN o remove_j\<close>
+  :: \<open> isasat_assn\<^sup>d \<rightarrow>\<^sub>a j_assn \<times>\<^sub>a isasat_assn\<close>
+  unfolding remove_j_def RETURN_case_isasat_int_invers
+  by sepref
+
+sepref_definition remove_k_code
+  is \<open>RETURN o remove_k\<close>
+  :: \<open> isasat_assn\<^sup>d \<rightarrow>\<^sub>a k_assn \<times>\<^sub>a isasat_assn\<close>
+  unfolding remove_k_def RETURN_case_isasat_int_invers
+  by sepref
+
+sepref_definition remove_l_code
+  is \<open>RETURN o remove_l\<close>
+  :: \<open> isasat_assn\<^sup>d \<rightarrow>\<^sub>a l_assn \<times>\<^sub>a isasat_assn\<close>
+  unfolding remove_l_def RETURN_case_isasat_int_invers
+  by sepref
+
+sepref_definition remove_m_code
+  is \<open>RETURN o remove_m\<close>
+  :: \<open> isasat_assn\<^sup>d \<rightarrow>\<^sub>a m_assn \<times>\<^sub>a isasat_assn\<close>
+  unfolding remove_m_def RETURN_case_isasat_int_invers
+  by sepref
+
+sepref_definition remove_n_code
+  is \<open>RETURN o remove_n\<close>
+  :: \<open> isasat_assn\<^sup>d \<rightarrow>\<^sub>a n_assn \<times>\<^sub>a isasat_assn\<close>
+  unfolding remove_n_def RETURN_case_isasat_int_invers
+  by sepref
+
+sepref_definition remove_o_code
+  is \<open>RETURN o remove_o\<close>
+  :: \<open> isasat_assn\<^sup>d \<rightarrow>\<^sub>a o_assn \<times>\<^sub>a isasat_assn\<close>
+  unfolding remove_o_def RETURN_case_isasat_int_invers
+  by sepref
+
+sepref_definition remove_p_code
+  is \<open>RETURN o remove_p\<close>
+  :: \<open> isasat_assn\<^sup>d \<rightarrow>\<^sub>a p_assn \<times>\<^sub>a isasat_assn\<close>
+  unfolding remove_p_def RETURN_case_isasat_int_invers
+  by sepref
+
+end
+
+
+context isasat_state
+begin
+lemma reconstruct_isasat[sepref_frame_match_rules]:
+  \<open>hn_ctxt
+     (isasat_int_assn (a_assn) (b_assn) (c_assn) (d_assn) (e_assn)
+    (f_assn) (g_assn) (h_assn) (i_assn) (j_assn) (k_assn)
+   (l_assn) (m_assn) (n_assn) (o_assn) (p_assn)) ax bx \<turnstile> hn_ctxt isasat_assn ax bx\<close>
+    unfolding isasat_assn_def
+    apply (auto split: prod.split isasat_int.splits elim: is_pureE
+      simp: sep_algebra_simps pure_part_pure_conj_eq)
+      done
+
+context
+  fixes x_assn :: \<open>'r \<Rightarrow> 'q \<Rightarrow> assn\<close> and
+    read_all_code :: \<open>'xa \<Rightarrow> 'xb \<Rightarrow> 'xc \<Rightarrow> 'xd \<Rightarrow> 'xe \<Rightarrow> 'xf \<Rightarrow> 'xg \<Rightarrow> 'xh \<Rightarrow> 'xi \<Rightarrow> 'xj \<Rightarrow> 'xk \<Rightarrow> 'xl \<Rightarrow> 'xm \<Rightarrow> 'xn \<Rightarrow> 'xo \<Rightarrow> 'xp \<Rightarrow> 'q llM\<close> and
+    read_all :: \<open>'a \<Rightarrow> 'b \<Rightarrow> 'c \<Rightarrow> 'd \<Rightarrow> 'e \<Rightarrow> 'f \<Rightarrow> 'g \<Rightarrow> 'h \<Rightarrow> 'i \<Rightarrow> 'j \<Rightarrow> 'k \<Rightarrow> 'l \<Rightarrow> 'm \<Rightarrow> 'n \<Rightarrow> 'o \<Rightarrow> 'p \<Rightarrow> 'r nres\<close>
+begin
+
+definition read_all_st_code :: \<open>_\<close> where
+  \<open>read_all_st_code xi = (case xi of
+  IsaSAT_int a1 a2 a3 a4 a5 a6 a7 a8 a9 a10 a11 a12 a13 a14 a15 a16 \<Rightarrow>
+    read_all_code a1 a2 a3 a4 a5 a6 a7 a8 a9 a10 a11 a12 a13 a14 a15 a16)\<close>
+
+definition read_all_st :: \<open>('a, 'b, 'c, 'd, 'e, 'f, 'g, 'h, 'i, 'j,
+     'k, 'l, 'm, 'n, 'o, 'p) isasat_int \<Rightarrow> _\<close> where
+  \<open>read_all_st isasat_int = (case isasat_int of IsaSAT_int a1 a2 a3 a4 a5 a6 a7 a8 a9 a10 a11 a12 a13 a14 a15 a16 \<Rightarrow>
+  read_all a1 a2 a3 a4 a5 a6 a7 a8 a9 a10 a11 a12 a13 a14 a15 a16)\<close>
+
+context
+  fixes P
+  assumes trail_read[sepref_fr_rules]: \<open>(uncurry15 read_all_code, uncurry15 read_all) \<in>
+      [uncurry15 P]\<^sub>a a_assn\<^sup>k *\<^sub>a b_assn\<^sup>k *\<^sub>a c_assn\<^sup>k *\<^sub>a d_assn\<^sup>k *\<^sub>a e_assn\<^sup>k *\<^sub>a f_assn\<^sup>k *\<^sub>a
+          g_assn\<^sup>k *\<^sub>a h_assn\<^sup>k *\<^sub>a i_assn\<^sup>k *\<^sub>a j_assn\<^sup>k *\<^sub>a k_assn\<^sup>k *\<^sub>a l_assn\<^sup>k *\<^sub>a
+          m_assn\<^sup>k *\<^sub>a n_assn\<^sup>k *\<^sub>a o_assn\<^sup>k *\<^sub>a p_assn\<^sup>k  \<rightarrow> x_assn\<close>
+  notes [[sepref_register_adhoc read_all]]
+begin
+sepref_definition read_all_code_tmp
+  is read_all_st
+  :: \<open>[case_isasat_int P]\<^sub>a isasat_assn\<^sup>k \<rightarrow> x_assn\<close>
+   unfolding read_all_st_def
+   by sepref
+
+lemmas read_all_code_refine =
+  read_all_code_tmp.refine[unfolded read_all_code_tmp_def
+    read_all_st_code_def[symmetric]]
+end
+
+end
+
+lemmas [unfolded Let_def, tuple16_getters_setters] =
+  update_a_def
+  update_b_def
+  update_c_def
+  update_d_def
+  update_e_def
+  update_f_def
+  update_g_def
+  update_h_def
+  update_i_def
+  update_j_def
+  update_k_def
+  update_l_def
+  update_m_def
+  update_n_def
+  update_o_def
+  update_p_def
+
+  remove_a_def
+  remove_b_def
+  remove_c_def
+  remove_d_def
+  remove_e_def
+  remove_f_def
+  remove_g_def
+  remove_h_def
+  remove_i_def
+  remove_j_def
+  remove_k_def
+  remove_l_def
+  remove_m_def
+  remove_n_def
+  remove_o_def
+  remove_p_def
+
+end
+
+lemmas [tuple16_getters_setters] =
+  isasat_state_ops.remove_a_def
+  isasat_state_ops.remove_b_def
+  isasat_state_ops.remove_c_def
+  isasat_state_ops.remove_d_def
+  isasat_state_ops.remove_e_def
+  isasat_state_ops.remove_f_def
+  isasat_state_ops.remove_g_def
+  isasat_state_ops.remove_h_def
+  isasat_state_ops.remove_i_def
+  isasat_state_ops.remove_j_def
+  isasat_state_ops.remove_k_def
+  isasat_state_ops.remove_l_def
+  isasat_state_ops.remove_m_def
+  isasat_state_ops.remove_n_def
+  isasat_state_ops.remove_o_def
+  isasat_state_ops.remove_p_def
+
+end
